Algebra/Functor.v
@@ -147,6 +147,57 @@ Section ComposeFunctor.
 
 End ComposeFunctor.
 
+Section ConstFunctor.
+  Inductive ConstFunc B {BS : Setoid B} A {AS : Setoid A} := ConstIso : B -> ConstFunc B A.
+
+  Instance ConstS {B} (BS : Setoid B) {A} (AS : Setoid A) : Setoid (ConstFunc B A) :=
+    {
+      equiv a b := match a, b with
+                     | ConstIso _ _ a', ConstIso _ _ b' => a'== b'
+                   end
+    }.
+  Proof.
+    split.
+    autounfold. intros. destruct x. reflexivity.
+    autounfold. intros. destruct x, y. symmetry. auto.
+    autounfold. intros. destruct x, y, z. transitivity b0. auto. auto.
+  Defined.
+  
+  Definition ConstIso' B {BS : Setoid B} A {AS : Setoid A} (a : ConstFunc B A) :=
+    match a with
+      | ConstIso _ _ a' => a'
+    end.
+  
+  Instance ConstIsoS_Proper  {B} {BS : Setoid B} {A} {AS : Setoid A} : Proper (equiv ==> equiv) (ConstIso B A).
+  Proof.
+    autounfold. intros. simpl. auto.
+  Qed.
+
+  Definition ConstIsoS {B} (BS : Setoid B) {A} (AS : Setoid A) : BS ~> ConstS BS AS :=
+    injF  (ConstIso B A) _.
+
+  Instance ConstIso'_Proper {B} {BS : Setoid B} {A} {AS : Setoid A}:  Proper (equiv ==> equiv) (ConstIso' B A).
+  Proof.
+    autounfold. unfold ConstIso'. intros. destruct x, y.  auto. 
+  Qed.
+
+  Definition ConstIsoS' {B} (BS : Setoid B) {A} (AS : Setoid A) : ConstS BS AS ~> BS := injF  (ConstIso' B A) _.
+
+  Definition constFunc_fmap {C} {CS : Setoid C} {A B} {AS : Setoid A} {BS : Setoid B} :
+    (AS ~~> BS) ~> (ConstS CS AS ~~> ConstS CS BS) :=
+    constS (AS ~~> BS) @ (ConstIsoS CS BS ∘ ConstIsoS' CS AS).
+
+  Instance ConstFunctor B (BS : Setoid B) : @Functor (ConstFunc B) (@ConstS B BS).
+  Proof.
+
+    exists (@constFunc_fmap B BS).
+    
+    intros. simpl. arrequiv. 
+    intros. simpl. arrequiv. destruct a. simpl. reflexivity.
+  Defined.
+
+End ConstFunctor.
+
 Notation "a <$> b" := (fmap  @ a @ b) (at level 49, left associativity).
 
 Section Utils.
