Assert.v
@@ -4,93 +4,90 @@ Require Import Tactics Utils Algebra.SetoidUtils Algebra.SetoidCat Algebra.ListU
 
 Require Import FMapWeakList List RelationClasses Relation_Definitions Morphisms SetoidClass.
 
-Module Type BuiltInPred.
-  Parameter app : builtinS ~> listS valS ~~> optionS boolS.
-End BuiltInPred.
 
-Inductive assertion :=
-| emp : assertion
-| singleton : expr -> pred -> expr -> assertion
-| sepConj : assertion -> assertion -> assertion
-| sepImp : assertion -> assertion -> assertion
-| atrue : assertion
-| aAnd : assertion -> assertion -> assertion
-| aNot : assertion -> assertion
-| aExists : var -> assertion -> assertion
-.
+Section Assert.
+  Context
+    {val : Type}
+    {builtin : Type}.
 
-Program Instance assertionS : Setoid assertion.
+  Definition expr := @expr val builtin.
 
-Notation "a & b" := (aAnd a b) (left associativity, at level 81).
-Notation "! a" := (aNot a) (at level 80).
-Notation "[[ addr , p ]] ⟼ val" := (singleton addr p val) (at level 79).
-Notation "a ∗ b" := (sepConj a b) (left associativity, at level 82).
-Notation "a -∗ b" := (sepImp a b) (right associativity, at level 83).
-Notation "'aexists' v , a" := (aExists v a) (at level 85).
+  Inductive assertion :=
+  | emp : assertion
+  | singleton : expr -> pred -> expr -> assertion
+  | sepConj : assertion -> assertion -> assertion
+  | sepImp : assertion -> assertion -> assertion
+  | atrue : assertion
+  | aAnd : assertion -> assertion -> assertion
+  | aNot : assertion -> assertion
+  | aExists : var -> assertion -> assertion
+  .
 
-Module Models (B: BuiltInExpr) (S : Store) (H : Heap).
-  Module EM := ExprModel B S.
-  Import EM S H.
+  Program Instance assertionS : Setoid assertion.
 
-  Reserved Notation "_⟦ a ⟧" (at level 20).
+
+End Assert.
+
+  Notation "a & b" := (aAnd a b) (left associativity, at level 81).
+  Notation "! a" := (aNot a) (at level 80).
+  Notation "[[ addr , p ]] ⟼ val" := (singleton addr p val) (at level 79).
+  Notation "a ∗ b" := (sepConj a b) (left associativity, at level 82).
+  Notation "a -∗ b" := (sepImp a b) (right associativity, at level 83).
+  Notation "'aexists' v , a" := (aExists v a) (at level 85).
+  
+Module AssertModel (VT : ValType) (B: BuiltInExpr VT) (S : Store VT) (H : Heap VT).
+  Module EM := ExprModel VT B S.
+  Module HU := HeapUtils VT H.
+  Import VT EM S H HU.
+  Definition assertion := @assertion val B.builtInExpr.
+  Instance assertionS : Setoid assertion := @assertionS val B.builtInExpr.
 
   Fixpoint _models (a : assertion) (s : S.t) (h : H.t) {struct a} : Prop :=
     match a with
-      | emp => H.dom @ h == ∅
+      | emp => ~exists a, inDom @ a @ h
       | [[ expr , pred ]] ⟼ expr2 => exists val val2,
                    ⟦ expr ⟧expr s == Some val /\
                    ⟦ expr2 ⟧expr s == Some val2 /\
-                   H.dom @ h == ﹛val﹜ /\
-                   H.preds @ h == ﹛pred﹜ /\
-                   h [val,pred] == Some val2
+                   singleton @ val @ pred @ val2 @ h
       | a0 ∗ a1 => exists h0 h1,
-                     h0 ⊥ h1 /\ h0 ⋅ h1 == h /\ _⟦ a0 ⟧ s h0  /\ _⟦ a1 ⟧ s h1
+                     h0 ⊥ h1 /\ h0 ⋅ h1 == h /\ _models a0 s h0  /\ _models a1 s h1
       | a0 -∗ a1 => forall h',
-                      h ⊥ h' -> _⟦ a0 ⟧ s h' -> _⟦ a1 ⟧ s (h ⋅ h') 
-      | ! a => ~ _⟦ a ⟧ s h
-      | a0 & a1 => _⟦ a0 ⟧ s h /\ _⟦ a1 ⟧ s h
+                      h ⊥ h' -> _models a0 s h' -> _models a1 s (h ⋅ h') 
+      | ! a => ~ _models a s h
+      | a0 & a1 => _models a0 s h /\ _models a1 s h
       | atrue => True
-      | aexists v, a => exists val, _⟦ a ⟧ (s [v ↦ val]s) h
-    end
-  where "_⟦ a ⟧" := (_models a).
+      | aexists v, a => exists val, _models a (S.update @ v @ val @ s) h
+    end.
 
   Definition models : assertionS ~> S.tS ~~> H.tS ~~> iff_setoid.
-    simple refine (injF (fun a=> injF2 (fun s h => _models a s h) _) _).
-Hint Unfold injF2. 
-    Lemma models_1 : forall a, Proper (equiv ==> equiv ==> equiv) (fun (s : S.t) (h : t) => (_⟦ a ⟧) s h).
+    simple refine (injF3 _models _).
+    Lemma models_1 : Proper (equiv ==> equiv ==> equiv ==> equiv) _models.
     Proof.
-      repeat autounfold. induction a.
-      intros. simpl.  rewrite H0.  tauto.
-      intros. unfold _models. destruct exprEval.      simpl. split.
-      intros. repeat destruct H1. destruct H2. destruct H3. destruct H4. exists x2. exists x3. split. assert (x1 x @ e == x1 y @ e). rewrite H. reflexivity. destruct (x1 x @ e), (x1 y @ e).  transitivity v. symmetry. auto. auto. auto. tauto. auto. split. assert (x1 x @ e0 == x1 y @ e0). rewrite H. reflexivity. destruct (x1 x @ e0), (x1 y @ e0). transitivity v. symmetry. auto. auto. auto. tauto. auto. split. rewrite <- H0. auto. split. rewrite <- H0. auto. assert (x0 [x2, p] == y0 [x2, p]). rewrite H0. reflexivity. destruct (x0 [x2, p]), (y0 [x2, p]). transitivity v. symmetry. auto. auto. auto. tauto. auto.
-      intros. repeat destruct H1. destruct H2. destruct H3. destruct H4. exists x2. exists x3. split. assert (x1 x @ e == x1 y @ e). rewrite H. reflexivity. destruct (x1 x @ e), (x1 y @ e).  transitivity v0. auto. auto. tauto. auto. auto. split. assert (x1 x @ e0 == x1 y @ e0). rewrite H. reflexivity. destruct (x1 x @ e0), (x1 y @ e0). transitivity v0. auto. auto. tauto. auto. auto. split. rewrite  H0. auto. split. rewrite  H0. auto. assert (x0 [x2, p] == y0 [x2, p]). rewrite H0. reflexivity. destruct (x0 [x2, p]), (y0 [x2, p]). transitivity v0.  auto. auto. tauto. auto. auto.
+      autounfold. intros x y H. rewrite H. clear x H. induction y.
+      intros. simpl.  split.
+      intros. intro. apply H1. destruct H2. destruct H2.  destruct H2. exists x1. exists x2. exists x3. equiv (x0 [x1, x2]) ( y0 [x1, x2]). simpl in H3. transitivity v0. auto. auto. auto.
+      intros. intro. apply H1. destruct H2. destruct H2.  destruct H2. exists x1. exists x2. exists x3. equiv (x0 [x1, x2]) ( y0 [x1, x2]). simpl in H3. transitivity v. symmetry. auto. auto. auto.
+      intros. unfold _models. split.
+      intro. destruct H1. destruct H1. exists x1. exists x2. rewrite <- H. rewrite <- H0. split. tauto. split. tauto. tauto. 
+      intro. destruct H1. destruct H1. exists x1. exists x2. rewrite H. rewrite H0. split. tauto. split. tauto. tauto. 
       intros. simpl. split.
-      intros. repeat destruct H1. exists x1. exists x2. rewrite <- (IHa1 _ _ H x1 x1) , <- (IHa2 _ _ H x2 x2). rewrite <- H0. auto. reflexivity. reflexivity. 
-      intros. repeat destruct H1. exists x1. exists x2. rewrite (IHa1 _ _ H x1 x1) , (IHa2 _ _ H x2 x2). rewrite H0. auto. reflexivity. reflexivity. 
-
-      intros. simpl. split.
-      intros. rewrite <- (IHa2 _ _ H (x0 ⋅ h') (y0 ⋅ h')). apply H1. rewrite H0. auto. rewrite (IHa1 _ _ H h' h'). auto. reflexivity. rewrite H0. reflexivity.
-      intros. rewrite (IHa2 _ _ H (x0 ⋅ h') (y0 ⋅ h')). apply H1. rewrite <- H0. auto. rewrite <- (IHa1 _ _ H h' h'). auto. reflexivity. rewrite H0. reflexivity.
-
+      intros. destruct H1. destruct H1. exists x1. exists x2. rewrite <- (IHy1 x y H x1 x1 (reflexivity x1)) , <- (IHy2 x y H x2 x2 (reflexivity x2)). rewrite <- H0. auto. 
+      intros. destruct H1. destruct H1. exists x1. exists x2. rewrite (IHy1 x y H x1 x1 (reflexivity x1)) , (IHy2 x y H x2 x2 (reflexivity x2)). rewrite H0. auto. 
+      intros. unfold _models. fold _models. split.
+      intros. rewrite <- (IHy2 _ _ H (x0 ⋅ h') (y0 ⋅ h')). apply H1. rewrite H0. auto. rewrite (IHy1 _ _ H h' h'). auto. reflexivity. rewrite H0. reflexivity.
+      intros. rewrite (IHy2 _ _ H (x0 ⋅ h') (y0 ⋅ h')). apply H1. rewrite <- H0. auto. rewrite <- (IHy1 _ _ H h' h'). auto. reflexivity. rewrite H0. reflexivity.
       intros. simpl. tauto.
-      intros. simpl. rewrite (IHa1 _ _ H _ _ H0), (IHa2 _ _ H _ _ H0). tauto.
-      intros. simpl. rewrite (IHa _ _ H _ _ H0). tauto.
+      intros. simpl. rewrite (IHy1 _ _ H _ _ H0), (IHy2 _ _ H _ _ H0). tauto.
+      intros. simpl. rewrite (IHy _ _ H _ _ H0). tauto.
       intros. simpl. split.
-      intros. destruct H1. exists x1. assert (x [v ↦ x1 ]s == y [v ↦ x1 ]s). rewrite H. reflexivity. rewrite <- (IHa (x [v ↦ x1 ]s) (y [v ↦ x1 ]s) H2 x0 y0 H0).  auto.
-      intros. destruct H1. exists x1. assert (x [v ↦ x1 ]s == y [v ↦ x1 ]s). rewrite H. reflexivity. rewrite(IHa (x [v ↦ x1 ]s) (y [v ↦ x1 ]s) H2 x0 y0 H0). auto.
+      intros. destruct H1. exists x1. assert (x [v ↦ x1 ]s == y0 [v ↦ x1 ]s). rewrite H. reflexivity. rewrite <- (IHy (x [v ↦ x1 ]s) (y0 [v ↦ x1 ]s) H2 x0 y1 H0).  auto.
+      intros. destruct H1. exists x1. assert (x [v ↦ x1 ]s == y0 [v ↦ x1 ]s). rewrite H. reflexivity. rewrite (IHy (x [v ↦ x1 ]s) (y0 [v ↦ x1 ]s) H2 x0 y1 H0). auto.
     Qed.
     apply models_1.
-    Lemma models_2 : forall pr, Proper (equiv ==> equiv)
-     (fun a : assertion =>
-        injF2 (fun (s : S.t) (h : t) => (_⟦ a ⟧) s h) (pr a)).
-    Proof.
-      repeat autounfold. intros. arrequiv.
-    Qed.
-    apply models_2.
   Defined.
   Notation "⟦ a ⟧" := (fun s h => models @ a @ s @ h) (at level 50, left associativity).
   Definition simply a a2 := forall s h, ⟦ a ⟧ s h -> ⟦ a2 ⟧ s h.
   Notation "a ⇒ a2" := (simply a a2) (at level 50).  
-End Models.  
+End AssertModel.  
 
 
