Definitions.v
@@ -1,6 +1,9 @@
+Require Import FSetInterface.
 Require Import Tactics Utils Algebra.SetoidUtils Algebra.SetoidCat  Algebra.Monad Algebra.PairUtils Algebra.Maybe Algebra.Alternative Algebra.Functor Algebra.FoldableFunctor Algebra.Applicative.
 
 Require Import FMapWeakList  RelationClasses Relation_Definitions Morphisms SetoidClass.
+
+Require Import Coq.Structures.DecidableTypeEx.
 
 
 Module FVarSet := FSetNat.
@@ -13,18 +16,11 @@ Definition var := nat.
 
 Definition pred := nat.
 
-Definition val := nat.
+Definition type := nat.
 
-Definition addr := nat.
-
-Definition builtin := nat.
-
-Program Instance natSetoid : Setoid nat.
-
-Instance varS : Setoid var := natSetoid.
-Instance valS : Setoid val := natSetoid.
-Instance predS : Setoid pred := natSetoid.
-Instance builtinS : Setoid builtin := natSetoid.
+Instance varS : Setoid var := natS.
+Instance predS : Setoid pred := natS.
+Instance typeS : Setoid type := natS.
 
 Program Instance natSetSetoid : Setoid FSetNat.t :=
   {
@@ -32,21 +28,38 @@ Program Instance natSetSetoid : Setoid FSetNat.t :=
   }.
 
 Instance varSetS : Setoid FVarSet.t := natSetSetoid.
-Instance valSetS : Setoid FValSet.t := natSetSetoid.
 Instance predSetS : Setoid FPredSet.t := natSetSetoid.
 
-Module Type Store.
+
+Module WSNotations (VT : WS).
+  Notation "∅" := VT.empty.
+  Notation "a ∩ b" := (VT.inter a b) (at level 11, left associativity).
+  Notation "a ∪ b" := (VT.union a b) (at level 12, left associativity).
+  Notation "﹛ a ﹜" := (VT.singleton a) (at level 10).
+  Notation "a ∈ b" := (VT.In a b) (at level 15).
+  Notation "a ∈? b" := (VT.mem a b) (at level 15).
+
+End WSNotations.
+
+Module Type ValType.
+  Parameter val : Type.
+  Parameter valS : Setoid val.
+  Axiom equiv_dec : forall val1 val2, {val1 == val2} + {~ val1 == val2}.
+End ValType.
+
+
+Module Type Store (VT : ValType).
+  Import VT.
   Parameter t : Type.
   Parameter tS : Setoid t.
   Parameter read : varS ~> tS ~~> optionS valS.
   Parameter update : varS ~> valS ~~> tS ~~> tS.
   Parameter delete : varS ~> tS ~~> tS.
   Parameter emptyStore : t.
-  Parameter dom : tS ~> varSetS.
   Notation "store [ var ↦ val ]s " := (update @ var @ val @ store) (at level 11).
   Notation "store [ var ]s " := (read @ var @ store) (at level 11).
 
-  Axiom eq_store : forall s1 s2, (forall v, read @ s1 @ v == read @ s2 @ v) -> s1 == s2.
+  Axiom eq_store : forall s1 s2, (forall v, read @ v @ s1 == read @ v @ s2) -> s1 == s2.
   (* Global Program Instance storesSetoid : Setoid (list t) := listS St.  *)
 
 (*  Instance eq_stores_Proper : Proper (eq_stores ==> eq_stores ==> iff) eq_stores.
@@ -78,18 +91,22 @@ Module Type Store.
   
   Axiom read_update_diff_var :
     forall s var var2 val,
+      var <> var2 ->
       s [ var ↦ val ]s [ var2 ]s == s [ var2 ]s.
 
   Axiom update_update_diff_var :
     forall s var var2 val val2,
+      var <> var2 ->
       s [ var ↦ val ]s [ var2 ↦ val2 ]s == s [ var2 ↦ val2 ]s [ var ↦ val ]s.
 
   Axiom delete_update_diff_var:
     forall s var var2 val,
+      var <> var2 ->
       delete @ var2 @ (s [ var ↦ val ]s) == (delete @ var2 @ s) [ var ↦ val ]s.
  
   Axiom read_delete_diff_var :
     forall s var var2,
+      var <> var2 ->
       (delete @ var @ s) [var2]s == s[var2]s.
 
   Axiom read_delete :
@@ -103,97 +120,71 @@ Module Type Store.
 
 End Store.
 
-Module Type Heap.
+Module Type Heap (VT : ValType).
+  Import VT.
   Open Scope type_scope.
   Parameter t : Type.
+  Parameter tS : Setoid t.
+  Parameter predOfType : predS ~> typeS ~~> tS ~~> iff_setoid.
+  Parameter typeOfHeap : typeS ~> tS ~~> iff_setoid.
+  Parameter newAddr : typeS ~> tS ~~> optionS (tS ~*~ valS).
+  Parameter allocated : valS ~> tS ~~> iff_setoid.
+  Parameter update : valS ~> predS ~~> valS ~~> tS ~~> tS.
+  Parameter delete : valS ~> tS ~~> tS.
+  Parameter emptyH : t.
+  Parameter readType : valS ~> tS ~~> optionS typeS.
+  Parameter read : valS ~> predS ~~> tS ~~> optionS valS.
+  Parameter union : tS ~> tS ~~> tS.
   Parameter l : forall A, (Setoid A) -> Type.
   Parameter lS : forall A (AS : Setoid A), Setoid (l A AS).
   Parameter (func : @Functor l lS).
   Parameter (alt : @Alternative l lS).
   Parameter (foldable : @FoldableFunctor l lS func).
   Parameter (app : @Applicative l lS func).
-  Parameter tS : Setoid t.
-  Parameter dom : tS ~> valSetS.
-  Parameter predDom : predS ~> tS ~~> valSetS.
-  Parameter preds : tS ~> predSetS.
-  Parameter newAddr : tS ~> (tS ~*~ valS).
-  Parameter delete : valS ~> tS ~~> tS.
-  Parameter deletePred :  valS ~> predS ~~> tS ~~> tS.
-  Parameter lookupBySPO :  valS ~> predS ~~> valS ~~> tS ~~> boolS.
-  Parameter lookupBySubject : valS ~> predS ~~> tS ~~> optionS valS.
   Parameter lookupByObject : predS ~> valS ~~> tS ~~> lS _ valS.
   Parameter lookupByPred : predS ~> tS ~~> lS _ (valS ~*~ valS).
-  Parameter update : valS ~> predS ~~> valS ~~> tS ~~> tS.
-  Parameter emptyH : t.
-  Parameter union : tS ~> tS ~~> tS.
 
-  Axiom eq_heap : forall (h1 h2 : t) , (forall v p, lookupBySubject @ v @ p @ h1 == lookupBySubject @ v @ p @ h2) -> h1 == h2.
-
-  Definition disjoint : tS ~> tS ~~> iff_setoid.
-   refine (injF2 (fun h1 => fun h2 => (dom @ h1) ∩ (dom @ h2) == ∅) _).
-   Lemma disjoint_1 : Proper (equiv ==> equiv ==> equiv)
-     (fun h1 h2 : t => (dom @ h1) ∩ (dom @ h2) == ∅).
-   Proof.
-     repeat     autounfold. intros. destruct dom. simpl in *.  
-                                                               
-     rewrite H, H0. reflexivity.  
-   Qed.
-   apply disjoint_1.
-  Defined.
-  
-  Notation "heap [ val , pred ]" := (lookupBySubject @ val @ pred @ heap) (at level 11).
+  Notation "heap [ val , pred ]" := (read @ val @ pred @ heap) (at level 11).
   Notation "heap [ val , pred  ↦  val2 ]  " := (update @ val @ pred @ val2 @ heap) (at level 11).
-  Notation "h1 ⊥ h2" := (disjoint @ h1 @ h2) (at level 15).
-  Notation "h1 ⋅ h2" := (union @ h1 @ h2) (at level 15).
 
-  Axiom dom_lookup : forall h val, val ∈ (dom @ h) -> exists pred val2, h [val,pred] == Some val2.
+  Axiom eq_heap : forall (h1 h2 : t) ,
+                    (forall v, allocated @ v @ h1 == allocated @ v @ h2) ->
+                    (forall v p, read @ v @ p @ h1 == read @ v @ p @ h2) ->
+                    (forall p t, predOfType @ p @ t @ h1 <-> predOfType @ p @ t @ h2) ->
+                    (forall t, typeOfHeap @ t @ h1 <-> typeOfHeap @ t @ h2) ->
+                    h1 == h2.
 
-  Axiom dom_domPred : forall h val, val ∈ (dom @ h) -> exists pred, val ∈ (predDom @ pred @ h).
+  Axiom read_empty : forall val pred, emptyH [val,pred] == None.
 
-  Axiom domPred_lookup : forall h val pred, val ∈ (predDom @ pred @ h) -> exists val2, h[val, pred] == Some val2.
-
-  Axiom lookupBySubject_empty : forall val pred, emptyH [val,pred] == None.
-
-  Axiom lookupByObject_empty : forall pred val, lookupByObject @ pred @ val @ emptyH == empty.
-
-  Axiom lookupByPred_empty : forall pred , lookupByPred @ pred @ emptyH == empty.
-
-  Axiom lookupBySPO_empty : forall val pred val2, lookupBySPO @ val @ pred @ val2 @ emptyH == false.
+  Axiom read_newAddr_1:
+        forall h type1 pred1 addr h', Some (h', addr) == newAddr @ type1 @ h -> read @ addr @ pred1 @ h == None.
   
-  Axiom lookup_predDom : forall h val pred, (exists val2, lookupBySubject @ val @ pred @ h == Some val2) -> val ∈ (predDom @ pred @ h).
+  Axiom read_newAddr_2:
+    forall h type1 pred1 addr h', Some (h', addr) == newAddr @ type1 @ h -> read @ addr @ pred1 @ h' == None.
 
-  Axiom predDom_dom : forall h val, (exists pred, val ∈ (predDom @ pred @ h)) -> val ∈ (dom @ h).
+  Axiom read_1 :
+    forall h val pred,
+      readType @ val @ h == None -> 
+      h [ val , pred ] == None.
 
-  Lemma lookup_dom : forall h val, (exists pred val2, lookupBySubject @ val @ pred @ h == Some val2) -> val ∈ (dom @ h).
-  Proof.
-    intros. apply predDom_dom. destruct H as [? [? ?]]. exists x. apply lookup_predDom. exists x0.  auto.
-  Qed.
+  Axiom read_2 :
+    forall h val pred t,
+      readType @ val @ h == Some t -> 
+      ~ predOfType @ pred @ t @ h ->
+      h [ val , pred ] == None.
 
-  Axiom predDom_newAddr:
-        forall h h' val pred, (h', val) == newAddr @ h -> val ∈? (predDom @ pred @ h) == false.
-  
-  Axiom lookupBySubject_predDom_0:
-        forall h val pred, val ∈? (predDom @ pred @ h) == false -> h [val , pred] == None.
-  
-  Axiom lookupBySubject_predDom_1:
-        forall h val pred, val ∈? (predDom @ pred @ h) == true -> exists val2, h [val , pred] == val2.
-
-  Lemma lookupBySubject_newAddr:
-        forall h h' val pred, (h', val) == newAddr @ h -> h [val, pred] == None.
-  Proof.
-    intros. apply lookupBySubject_predDom_0. apply predDom_newAddr with (h:=h) (h':=h'). auto.
-  Qed.
-  
-  Axiom lookup_update :
-    forall h val pred val2,
+  Axiom read_update :
+    forall h val pred val2 t,
+      readType @ val @ h == Some t -> 
+      predOfType @ pred @ t @ h ->
       h [ val , pred ↦  val2 ] [ val , pred ] == Some val2.
   
-  Axiom lookup_update_diff_addr :
+  Axiom read_update_diff_addr :
     forall h val val' pred pred' val2,
       val <> val' ->
       h [ val , pred ↦ val2 ] [ val' , pred' ] == h [ val' , pred' ].
   
-  Axiom lookup_update_diff_pred :
+  Axiom read_update_diff_pred :
     forall h val val' pred pred' val2,
       pred <> pred' ->
       h [ val , pred ↦ val2 ] [ val' , pred' ] == h [ val' , pred' ].
@@ -202,24 +193,89 @@ Module Type Heap.
     forall h val pred val2 val3,
       h [ val , pred ↦  val2 ] [ val , pred ↦ val3 ] == h  [ val , pred ↦ val3 ].
   
-  Axiom predDom_update :
-    forall h val pred val2,
-      val ∈? (predDom @ pred @ ( h [ val , pred ↦ val2 ])) == true.
-  
-  Axiom predDom_update_diff_addr :
-    forall h val val' pred pred' val2,
-      val <> val' -> 
-      val ∈? (predDom @ pred @ ( h [ val' , pred' ↦ val2 ])) == val ∈? (predDom @ pred @ h).
-
-  Axiom predDom_update_diff_pred :
-    forall h val val' pred pred' val2,
-      pred <> pred' -> 
-      val ∈? (predDom @ pred @ ( h [ val' , pred' ↦ val2 ])) = val ∈? (predDom @ pred @ h).
-
-  Axiom dom_update_diff_addr :
-    forall h val val' pred val2,
-      val <> val' -> 
-      val ∈? (dom @ ( h [ val' , pred ↦ val2 ])) == val ∈? (dom @ h).
-
 End Heap.
 
+Module HeapUtils (VT : ValType) (H : Heap VT).
+  Import VT H.
+
+  Definition lookupBySPO :  valS ~> predS ~~> valS ~~> tS ~~> boolS.
+    simple refine (injF4 (fun addr1 pred1 val1 h =>
+                            match h[addr1, pred1] with
+                              | Some val2 => if equiv_dec val1 val2 then true else false
+                              | None => false
+                            end) _).
+    Lemma lookupBySPO_1 : Proper (equiv ==> equiv ==> equiv ==> equiv ==> equiv)
+     (fun (addr1 : val) (pred1 : pred) (val1 : val) (h : t) =>
+      match h [addr1, pred1] with
+      | Some val2 => if equiv_dec val1 val2 then true else false
+      | None => false
+      end).
+    Proof.
+      autounfold. intros. matchequiv. simpl in H3. destruct (equiv_dec x1 v). destruct (equiv_dec y1 v0). reflexivity. destruct n. transitivity x1. symmetry. auto. transitivity v. auto. auto. destruct (equiv_dec y1 v0). destruct n. transitivity y1. auto. transitivity v0. auto. symmetry. auto. reflexivity.
+    Qed.
+    apply lookupBySPO_1.
+  Defined.
+    
+
+  Definition inDom : valS ~> tS ~~> iff_setoid.
+    simple refine (injF2 (fun addr h => exists pred1 a, read @ addr @ pred1 @ h == Some a) _).
+    apply optionS.
+    apply valS.
+    Lemma inDom_1 : Proper (equiv ==> equiv ==> equiv)
+     (fun (addr : val) (h : t) =>
+        exists (pred1 : pred) (a : val), h [addr, pred1] == Some a).
+    Proof.
+      solve_proper.
+    Qed.
+    apply inDom_1.
+  Defined.
+
+  Definition disjoint : tS ~> tS ~~> iff_setoid.
+   refine (injF2 (fun h1 h2 => forall addr, ~(inDom @ addr @ h1) \/ ~ (inDom @ addr @ h2)) _).
+   Lemma disjoint_1 : Proper (equiv ==> equiv ==> equiv)
+     (fun h1 h2 => forall addr, ~(inDom @ addr @ h1) \/ ~ (inDom @ addr @ h2)).
+   Proof.
+     solve_proper.     
+   Qed.
+   apply disjoint_1.
+  Defined.
+
+  Definition singleton : valS ~> predS ~~> valS ~~> tS ~~> iff_setoid.
+    simple refine (injF4 (fun addr1 pred1 val1 h =>
+                            h [ addr1 , pred1 ] == Some val1 /\
+                            forall addr2 pred2 val2,
+                              h [ addr2 , pred2 ] == Some val2 ->
+                              addr1 == addr2 /\
+                              pred1 == pred2 /\
+                              val2 == val1) _).
+    apply optionS.
+    apply valS.
+    apply optionS.
+    apply valS.
+    apply valS.
+    apply predS.
+    apply valS.
+    Lemma singleton_1 : Proper (equiv ==> equiv ==> equiv ==> equiv ==> equiv)
+     (fun (addr1 : val) (pred1 : pred) (val1 : val) (h : t) =>
+      h [addr1, pred1] == Some val1 /\
+      (forall (addr2 : val) (pred2 : pred) (val2 : val),
+       h [addr2, pred2] == Some val2 ->
+       addr1 == addr2 /\ pred1 == pred2 /\ val2 == val1)).
+    Proof.
+      autounfold. intros. rewrites. split.
+      intros. destruct H3. split.
+      rewrite H3. simpl. auto.
+      intros. rewrite <- H1, <- H.  apply H4. rewrite H2. auto.
+      intros. destruct H3. split.
+      rewrite H3. simpl. symmetry. auto.
+      intros. rewrite H1, H.  apply H4. rewrite <- H2. auto.
+    Qed.
+    apply singleton_1.
+  Defined.
+  
+  Notation "heap [ val , pred ]" := (read @ val @ pred @ heap) (at level 11).
+  Notation "heap [ val , pred  ↦  val2 ]  " := (update @ val @ pred @ val2 @ heap) (at level 11).
+  Notation "h1 ⊥ h2" := (disjoint @ h1 @ h2) (at level 15).
+  Notation "h1 ⋅ h2" := (union @ h1 @ h2) (at level 15).
+
+End HeapUtils.
