Expr.v
@@ -3,142 +3,68 @@ Require Import Tactics Utils Algebra.SetoidUtils Algebra.SetoidCat Algebra.ListU
 Require Import FMapWeakList List RelationClasses Relation_Definitions Morphisms SetoidClass.
 
 
+Section Expr.
+  Context
+    {val : Type}
+    {builtin : Type}.
 
-
-Inductive expr :=
+  Inductive expr :=
 | valExpr : val -> expr
 | varExpr : var -> expr
 | appExpr : builtin -> list expr -> expr
-.
+  .
 
-Program Instance exprS : Setoid expr :=
-  {
-    equiv := eq
-  }.
+  Program Instance exprS : Setoid expr :=
+    {
+      equiv := eq
+    }.
 
-Section ExprInductionPrinciple.
-  Variables (p : expr -> Prop) (Q : list expr -> Prop).
+  Section ExprInductionPrinciple.
+    Variables (p : expr -> Prop) (Q : list expr -> Prop).
 
-  Hypothesis
-    (pval : forall val, p (valExpr val))
-    (pvar : forall var, p (varExpr var))
-    (papp0 : Q List.nil)
-    (papp1 : forall e, p e -> forall l, Q l -> Q (e :: l))
-    (papp : forall builtin l, Q l -> p (appExpr builtin l)).
-  
-    Fixpoint expr_ind_2 e : p e :=
-    match e as x return p x with
-      | valExpr val => pval val
-      | varExpr var => pvar var
-      | appExpr builtin l =>
-        papp builtin l ((
-               fix dep_fold_right (l' : list expr) : Q l' :=
-                 match l' as x return Q x with
-                   | List.nil => papp0
-                   | e :: es => papp1 e (expr_ind_2 e) es (dep_fold_right es)
-                 end
-             ) l)
-    end.
-End ExprInductionPrinciple.
-
-Section ExprRecursionPrincipleNonDep.
-  Context {P : Type} {Q : Type}.
-
-  Hypothesis
-    (pval : val -> P)
-    (pvar : var -> P)
-    (papp0 : Q)
-    (papp1 : expr -> P -> list expr -> Q -> Q)
-    (papp : builtin -> list expr -> Q -> P).
-  
-    Fixpoint expr_rect_nondep_2 e : P :=
-    match e with
-      | valExpr val => pval val
-      | varExpr var => pvar var
-      | appExpr builtin l =>
-        papp builtin l ((
-               fix nondep_fold_right (l' : list expr) : Q :=
-                 match l' with
-                   | List.nil => papp0
-                   | e :: es => papp1 e (expr_rect_nondep_2 e) es (nondep_fold_right es)
-                 end
-             ) l)
-    end.
-
-    Context {SP : Setoid P} {SQ : Setoid Q}.
-
-    Definition expr_rect_nondep_2Proper  : exprS ~> SP.
-      simple refine (injF expr_rect_nondep_2 _).
-    Defined.
-    
-End ExprRecursionPrincipleNonDep.
-
-(* Section ExprIterationPrincipleNonDep.
-  Context {P : Type} {Q : Type}.
-
-
-  Section Raw.
     Hypothesis
-    (pval : val -> P)
-    (pvar : var -> P)
-    (papp0 : Q)
-    (papp1 : P -> Q -> Q)
-    (papp : builtin -> Q -> P).
-  
-    Fixpoint expr_itrt_nondep_2 (e : expr) : P :=
-    match e with
-      | valExpr val => pval val
-      | varExpr var => pvar var
-      | appExpr builtin l =>
-        papp builtin ((
-               fix nondep_fold_right (l' : list expr) : Q :=
-                 match l' with
-                   | List.nil => papp0
-                   | e :: es => papp1  (expr_itrt_nondep_2 e)  (nondep_fold_right es)
-                 end
-             ) l)
-    end.
-  End Raw.
-  
-  Context {SP : Setoid P} {SQ : Setoid Q}.
-
-  Definition expr_itrt_nondep_2Proper :
-    (valS ~~> SP) ~>
-    SP ~~>
-    SQ ~~>
-    (SP ~~> SQ ~~> SQ) ~~>
-    (builtinS ~~> SQ ~~> SP) ~~>
-    exprS ~~> SP.
-      simple refine (injF expr_itrt_nondep_2 _).
-
-      Lemma expr_itrt_nondep_2Proper_1 : properF expr_itrt_nondep_2.
-      Proof.
-        unfold properF. solve_proper.
-      Qed.
-
-      apply expr_itrt_nondep_2Proper_1.
-                                           Defined.
+      (pval : forall val, p (valExpr val))
+      (pvar : forall var, p (varExpr var))
+      (papp0 : Q List.nil)
+      (papp1 : forall e, p e -> forall l, Q l -> Q (e :: l))
+      (papp : forall builtin l, Q l -> p (appExpr builtin l)).
     
-    
-End ExprIterationPrincipleNonDep. *)
+    Fixpoint expr_ind_2 e : p e :=
+      match e as x return p x with
+        | valExpr val => pval val
+        | varExpr var => pvar var
+        | appExpr builtin l =>
+          papp builtin l ((fix dep_fold_right (l' : list expr) : Q l' :=
+                             match l' as x return Q x with
+                               | List.nil => papp0
+                               | e :: es => papp1 e (expr_ind_2 e) es (dep_fold_right es)
+                             end
+                          ) l)
+      end.
+  End ExprInductionPrinciple.
+
+  Fixpoint exprFreeVars expr :=
+    match expr with
+      | valExpr _ => FVarSet.empty
+      | varExpr var => FVarSet.singleton var
+      | appExpr builtin exprs =>  fold_right FVarSet.union FVarSet.empty (map exprFreeVars exprs)
+    end
+  .
+
+End Expr.
 
 
-Fixpoint exprFreeVars expr :=
-  match expr with
-    | valExpr _ => ∅
-    | varExpr var => ﹛ var ﹜
-    | appExpr builtin exprs =>  fold_right FSetNat.union ∅ (map exprFreeVars exprs)
-  end
-.
-
-
-
-Module Type BuiltInExpr.
-  Parameter app : builtinS ~> listS valS ~~> optionS valS.
+Module Type BuiltInExpr (VT : ValType).
+  Import VT.
+  Parameter builtInExpr : Type.
+  Parameter builtInExprS : Setoid builtInExpr.
+  Parameter appBIE : builtInExprS ~> listS valS ~~> optionS valS.
 End BuiltInExpr.
   
-Module ExprModel (B : BuiltInExpr) (S : Store).
-  Import S.
+Module ExprModel (VT : ValType) (B : BuiltInExpr VT) (S : Store VT).
+  Import VT S B.
+  Definition expr := @expr val builtInExpr.
+  Instance exprS : Setoid expr := @exprS val builtInExpr.
   Existing Instance maybe_Monad.
   Existing Instance monadFunctor.
   Existing Instance monad_Applicative.
@@ -154,24 +80,18 @@ Module ExprModel (B : BuiltInExpr) (S : Store).
                 | e :: es => consS <$> _exprEval s e <*> _exprsEval s es
               end) s args with
           | None => None
-          | Some l => B.app @ b @ l
+          | Some l => appBIE @ b @ l
         end
     end.
-
-  Lemma fold_right_cons : forall A B (f : A -> B -> B) (b : B) (a : A) (l : list A),
-                            fold_right f b (a :: l) = f a (fold_right f b l).
-  Proof.
-    reflexivity.
-  Qed.
   
   Definition exprEval : S.tS ~> exprS ~~> optionS valS.
     simple refine (
              injF2 _exprEval _).
     Lemma exprEval_1 :  Proper (equiv ==> equiv ==> equiv) _exprEval.
     Proof.
-      repeat autounfold. intros. simpl in H0. rewrite H0. clear H0 x0. generalize H. clear H. apply expr_ind_2 with (e:= y0) (Q:=fun es => allTrue (fun y0 => x == y -> _exprEval x y0 == _exprEval y y0) es).
-      intros. simpl. auto.
-      intros. simpl. equiv (x [var ]s) (y [var ]s) H. auto. 
+      autounfold. intros. simpl in H0. rewrite H0. clear H0 x0. generalize H. clear H. apply expr_ind_2 with (e:= y0) (Q:=fun es => allTrue (fun y0 => x == y -> _exprEval x y0 == _exprEval y y0) es).
+      intros. simpl. reflexivity.
+      intros. simpl. equiv (x [var ]s) (y [var ]s). auto. 
       compute. auto.
       intros. unfold allTrue. rewrite map_cons.  rewrite fold_right_cons. split.
       auto.
@@ -184,7 +104,7 @@ Module ExprModel (B : BuiltInExpr) (S : Store).
         end)). fold _es. assert (_es x l == _es y l).  induction l.
       simpl. constructor. 
       unfold _es. fold _es. destruct H. rewrite (IHl H1). rewrite (H H0). reflexivity.
-equiv (_es x l) (_es y l) H1. simpl in H1. rewrite H1. reflexivity. 
+equiv (_es x l) (_es y l). simpl in H1. rewrite H1. reflexivity. 
     Qed.
     apply exprEval_1.  
   Defined.
