Algebra/Lens/ListLens.v
@@ -1,0 +1,1020 @@
+Require Import Algebra.Functor Algebra.Applicative Algebra.SetoidCat Algebra.ListUtils Algebra.PairUtils Algebra.Maybe Algebra.SetoidUtils Algebra.Monad Algebra.Maybe Tactics Utils VectorUtils Algebra.Lens.LensTypes Algebra.Pointed.
+Require Import SetoidClass List Coq.Classes.RelationClasses Coq.Arith.PeanoNat Coq.Arith.Compare_dec.
+Import ListNotations.
+
+
+Instance length_Proper A (AS : Setoid A) : Proper (equiv ==> equiv) (@length A).
+  Proof.
+    autounfold. intros. generalize H. clear H. apply list_ind_2 with (l1:=x) (l2:=y).
+    reflexivity.
+    intros. inversion H0.
+    intros. inversion H0.
+    intros. simpl. rewrite H. auto. inversion H0. auto.
+  Qed.
+
+  Instance nth_error_Proper A (AS : Setoid A) : Proper (equiv ==> equiv ==> equiv) (@nth_error A).
+  Proof.
+    autounfold. intros. generalize H x0 y0 H0. clear H x0 y0 H0. apply list_ind_2 with (l1:=x) (l2:=y).
+    intros. rewritesr. 
+    intros. inversion H0.
+    intros. inversion H0.
+    intros. inversion H0. simpl. simpl in H1.  rewrite H1. destruct y0. simpl. auto.
+    simpl. apply H. auto. reflexivity.
+  Qed.
+
+Fixpoint listS_update {f fS func} {app : @Applicative f fS func} {A} {AS : Setoid A} (n:nat) (l:list A)  (t:AS ~>  fS _ AS) {struct n} :  f (list A) _ :=
+  match n, l with
+    | 0,   old_v::rest => consS <$> t @ old_v <*> pure @ rest
+    | S n, v'::rest    => consS <$> pure @ v' <*> listS_update n rest  t 
+    | _,   nil         => pure @ nil
+  end.
+
+
+Instance listS_update_Proper {f fS func} {app : @Applicative f fS func} A (AS : Setoid A): Proper (equiv ==> equiv ==> equiv ==> equiv) (listS_update).
+Proof.
+  autounfold. intros. rewrite H.  clear x H. generalize y H0. clear H0. apply list_ind_2 with (l1:=x0) (l2:=y0).
+  intros. induction y2.
+  simpl. evalproper. 
+  simpl. evalproper. 
+  intros. inversion H0.
+  intros. inversion H0.
+  intros. inversion H0. induction y2.
+  simpl. evalproper. evalproper. rewritesr. evalproper. evalproper. arrequiv. auto.
+  simpl. evalproper. evalproper. evalproper. evalproper. evalproper. evalproper. arrequiv. auto. 
+Qed.
+
+Definition list_updateS {f fS func} {app : @Applicative f fS func} {A} {AS : Setoid A} := injF3 (@listS_update f fS func app A AS) _.
+
+Fixpoint list_update' {A} {AS : Setoid A} (n:nat) (l:list A)  (a:A ) {struct n} :  list A :=
+  match n, l with
+    | 0,   old_v::rest => a :: rest
+    | S n, v'::rest    => v' :: list_update' n rest  a 
+    | _,   nil         => nil
+  end.
+
+
+Instance list_update'_Proper A (AS : Setoid A): Proper (equiv ==> equiv ==> equiv ==> equiv) (list_update').
+Proof.
+  autounfold. intros. rewrite H.  clear x H. generalize y H0. clear H0. apply list_ind_2 with (l1:=x0) (l2:=y0).
+  intros. induction y2.
+  simpl.  reflexivity. 
+  simpl. reflexivity. 
+  intros. inversion H0.
+  intros. inversion H0.
+  intros. inversion H0. induction y2.
+  simpl.  constructor.  auto. auto. 
+  simpl. constructor. auto. apply H. auto. 
+Qed.
+
+Definition list_updateS' {A} {AS : Setoid A} := injF3 (@list_update' A AS) _.
+
+Definition _nthTraversal' {A} {AS : Setoid A} (n : nat) : _Traversal' (list A) A.
+  unfold _Traversal'. intros. refine (match nth_error X0 n with
+                                    | None => pure @ X0
+                                    | Some a => listS_update n X0  X
+                                  end).
+Defined.
+
+Definition _nthTraversal {f fS func} {app : @Applicative f fS func} {A} {AS : Setoid A} (n : nat) :
+  (AS ~> fS _ AS) -> list A -> f (list A) _ := _nthTraversal' n f fS func app.
+
+Instance _nthTraversal_Proper {f fS func} {app : @Applicative f fS func} A (AS : Setoid A) : Proper (equiv ==> equiv ==> equiv ==> equiv) (_nthTraversal).
+Proof.
+  autounfold. intros. unfold _nthTraversal, _nthTraversal'. matchequiv. rewrite H. clear x H. generalize y H1. clear y H1. apply list_ind_2 with (l1:=x1) (l2:=y1).
+  intros. rewritesr. 
+  intros. inversion H1.
+  intros. inversion H1.
+  intros. inversion H1. induction y.
+  unfold listS_update. rewrite H0, H6, H8. reflexivity.
+  unfold listS_update. fold listS_update. rewrite H. rewrite H6. reflexivity. auto. rewritesr.
+Qed.
+
+Definition nthTraversal {f fS func} {app : @Applicative f fS func} {A} {AS : Setoid A} := injF3 _nthTraversal _.
+
+
+
+Fixpoint list_zipWith {A : Type} {AS : Setoid A} {B : Type} {BS : Setoid B}{C : Type} {CS : Setoid C}(f : AS ~> BS ~~> CS) (l1 : list A) (l2 : list B)  :=
+  match l1 , l2 with
+    | nil , _ => nil
+    | _, nil => nil
+    | a1 :: as1 , a2 :: as2 => (f @ a1 @ a2) :: list_zipWith f as1 as2 
+  end
+.
+
+Instance list_zipWith_Proper {A : Type} {AS : Setoid A} {B : Type} {BS : Setoid B}{C : Type} {CS : Setoid C} : Proper (equiv ==> equiv ==> equiv ==> equiv) (@list_zipWith A _ B _ C _).
+Proof.
+  autounfold. intros. generalize H0 x1 y1 H1. clear H0 x1 y1 H1. apply list_ind_2 with (l1:=x0) (l2:=y0).
+  intros. simpl. auto.
+  intros. inversion H1.
+  intros. inversion H1.
+  intros. inversion H1. simpl. matchequiv.
+  inversion H9.   constructor. auto. auto.
+rewritesr.
+  apply H0. auto. auto.
+Qed.
+
+Definition list_zipWithS {A : Type} {AS : Setoid A} {B : Type} {BS : Setoid B}{C : Type} {CS : Setoid C} := injF3 (@list_zipWith A _ B _ C _) _.
+
+Fixpoint list_zipWith' {A : Type} {AS : Setoid A} {B : Type} {BS : Setoid B} (f : AS ~> BS ~~> AS) (l1 :list A) (l2 : list B)  :=
+  match l1 , l2 with
+    | nil , _ => nil
+    | _, nil => l1
+    | a1 :: as1 , a2 :: as2 => (f @ a1 @ a2) :: list_zipWith' f as1 as2 
+  end
+.
+
+Instance list_zipWith'_Proper {A : Type} {AS : Setoid A}{B : Type} {BS : Setoid B} : Proper (equiv ==> equiv ==> equiv ==> equiv) (@list_zipWith' A _ B _).
+Proof.
+  autounfold. intros. generalize H0 x1 y1 H1. clear H0 x1 y1 H1. apply list_ind_2 with (l1:=x0) (l2:=y0).
+  intros. simpl. auto.
+  intros. inversion H1.
+  intros. inversion H1.
+  intros. inversion H1. simpl. matchequiv.
+  constructor. auto. auto.
+  inversion H9. constructor. rewritesr.
+  apply H0. auto. auto.
+Qed.
+
+
+Definition list_zipWithS' {A : Type} {AS : Setoid A} {B : Type} {BS : Setoid B} := injF3 (@list_zipWith' A _ B _) _.
+
+Definition nth_errorS {A : Type} {AS : Setoid A} : listS AS ~> natS ~~> maybeS AS := injF2 (@nth_error A) _.
+
+Definition nth_errorS' {A : Type} {AS : Setoid A} := flipS @ (@nth_errorS A AS).
+
+Lemma list_zipWith'_cons : forall {A : Type} {AS : Setoid A}{B : Type} {BS : Setoid B}(a : A) (la : list A) (b: B) (lb: list B)(f : AS ~> BS ~~> AS), list_zipWith' f (a::la)(b::lb) = (f @ a @ b) :: list_zipWith' f la lb.
+
+Proof.
+  intros. reflexivity.
+Qed.
+
+
+(* infinite list with finite nonrepeating prefix and an infinitely repeating element *)
+
+Inductive lista A : Type := listaCons : A -> list A -> @lista A.
+
+Fixpoint list_all {A} {AS : Setoid A} (l : list A) (a : A) :=
+  match l with
+    | nil => True
+    | a' :: l' => a' == a /\ list_all l' a
+  end.
+
+Fixpoint lista_equiv0 {A} {AS : Setoid A} (a1 a2 : A) (l1 l2 : list A) :=
+  match l1, l2 with
+    | nil, l2' => a1 == a2 /\ list_all l2' a1
+    | a1' :: l1', nil =>
+      a1' == a2 /\ lista_equiv0 a1 a2 l1' nil
+    | a1' :: l1', a2' :: l2' =>
+      a1' == a2' /\ lista_equiv0 a1 a2 l1' l2'
+  end
+.
+Lemma lista_equiv0_equiv : forall A (AS : Setoid A) (a1 a2 : A) (l1 l2 : list A), lista_equiv0 a1 a2 l1 l2 -> a1 == a2.
+Proof.
+  intros. generalize H. clear H. apply list_ind_2 with (l1:=l1)(l2:=l2).
+  simpl. tauto.
+  intros. simpl in *. tauto.
+  intros. simpl in *. tauto.
+  intros. simpl in *. tauto.
+Qed.
+
+                               
+Definition lista_equiv {A} {AS : Setoid A} (l1 l2 : lista A) :=
+  match l1, l2 with
+    | listaCons _ a1 ll1, listaCons _ a2 ll2 => lista_equiv0 a1 a2 ll1 ll2
+  end.
+
+Instance lista_equiv_Equivalence {A} {AS : Setoid A} : Equivalence (@lista_equiv A AS).
+Proof.
+  split.
+  autounfold. intros. destruct x. simpl. induction l.
+  simpl. split. reflexivity. auto.
+  simpl. split. reflexivity. auto. 
+  autounfold. intros. destruct x,y. simpl in *. generalize H. clear H. apply list_ind_2 with (l1:=l) (l2:=l0).
+  intros.   simpl. destruct H. split. symmetry. auto. auto.
+  intros.  simpl. simpl in H0. split.  tauto.  apply H. simpl.  tauto.
+  intros.  simpl. simpl in H0, H. split. apply H. tauto. split. tauto. apply H. tauto.
+  intros. simpl. simpl in H0. split. symmetry. tauto. apply H. tauto.
+  autounfold. intros. destruct x,y,z. simpl in *.  generalize l0 H H0. clear H l0 H0. apply list_ind_2 with (l1:=l) (l2:=l1).
+  intros. simpl in *. split. transitivity a0. tauto. apply lista_equiv0_equiv with (l1:=l0) (l2:=nil). auto. auto. 
+  intros. simpl in *. split. transitivity a0. tauto. apply lista_equiv0_equiv with (l1:=l0) (l2:=a2 :: b). auto. split. destruct l0. simpl in *. transitivity a0. tauto. symmetry. tauto. simpl in *. transitivity a3. symmetry. tauto. tauto. destruct l0.  specialize (H nil). simpl in *.  tauto. specialize (H l0). simpl in *. tauto.
+  intros. simpl in *. split. destruct l0. simpl in *. transitivity a0. tauto. tauto. transitivity a3. tauto. simpl in *. tauto. destruct l0. simpl in *. apply H with (l0:=nil).  tauto. auto. simpl in *. apply H with (l0:=l0). tauto. tauto.
+  intros. simpl in *. split. destruct l0. simpl in *. transitivity a0. tauto. symmetry. tauto. simpl in *. transitivity a3. tauto. tauto. destruct l0. simpl in *. apply H with (l0 := nil). tauto. simpl. tauto. simpl in *. apply H with (l0:=l0). tauto. tauto.
+Qed.
+
+Instance listaS {A} (AS : Setoid A) : Setoid (lista A) :=
+  {
+    equiv := lista_equiv
+  }.
+
+Fixpoint lista_update0 {A} {AS : Setoid A} (n:nat) (a0 : A) (l:list A)  (a:A ) {struct n} :  list A :=
+  match n, l with
+    | 0, [] => [a] 
+    | 0, a'::l' => a ::l'
+    | S n', [] => a0 :: lista_update0 n' a0 [] a
+    | S n', a'::l' => a':: lista_update0 n' a0 l' a
+  end.
+
+
+Instance lista_update0_Proper A (AS : Setoid A): Proper (equiv ==> equiv ==> equiv ==> equiv ==> equiv) (@lista_update0 A AS).
+Proof.
+  autounfold. intros. rewrite H.  clear x H. generalize y H1. clear y H1. apply list_ind_2 with (l1:=x1) (l2:=y1).
+  intros. induction y.
+  simpl.  constructor. auto. auto. 
+  simpl.  constructor. auto. auto. 
+  intros. inversion H1.
+  intros. inversion H1.
+  intros. inversion H1. induction y.
+  simpl.  constructor.  auto. auto. 
+  simpl. constructor. auto. apply H. auto. 
+Qed.
+
+Definition lista_update {A} {AS : Setoid A} (n:nat) (l:lista A)  (a:A )  :  lista A :=
+  match l with
+    | listaCons _ a0 l => listaCons _ a0 (lista_update0 n a0 l a)
+  end.
+
+Hint Unfold lista_update.
+
+Instance listaCons_Proper A (AS : Setoid A): Proper (equiv ==> equiv ==> equiv) (@listaCons A).
+Proof.
+  autounfold. intros. simpl. generalize H0. clear H0. apply list_ind_2 with (l1:=x0) (l2:=y0).
+  simpl. auto.
+  intros. inversion H1.
+  intros. inversion H1.
+  intros. inversion H1. simpl. tauto.
+Qed.
+
+Definition listaConsS {A} {AS : Setoid A} := injF2 (@listaCons A) _.
+Lemma listaCons_equiv : forall A (AS : Setoid A) (a1 a2 : A) (l1 l2 : list A), listaCons _ a1 l1 == listaCons _ a2 l2 -> a1 == a2.
+Proof.
+  intros. generalize H. clear H. apply list_ind_2 with (l1:=l1)(l2:=l2).
+  simpl. tauto.
+  intros. apply H. simpl in *. tauto.
+  intros. apply H. simpl in *. tauto.
+  intros. apply H. simpl in *. tauto.
+Qed.
+
+Instance lista_update_Proper A (AS : Setoid A): Proper (equiv ==> equiv ==> equiv ==> equiv) (@lista_update A AS).
+Proof.
+  autounfold. intros. destruct x0, y0.  rewrite H, H1. clear x H x1 H1. generalize y H0. clear y H0. apply list_ind_2 with (l1:=l) (l2:=l0).
+  intros. induction y.
+  simpl in *.   split. reflexivity. tauto. 
+  simpl in *.  tauto. 
+  intros. destruct y.
+  simpl in *. split. reflexivity. tauto.
+  simpl. simpl in H0.  split.   symmetry. tauto. apply H.  simpl. tauto.
+  intros. destruct y.
+  simpl in *. split. reflexivity. tauto.
+  simpl. simpl in H0. split. tauto. simpl in *. apply H. tauto. 
+  intros. destruct y.
+  simpl in *. split. reflexivity. tauto.
+  simpl in *. split. tauto. apply H. tauto.
+Qed.
+
+Definition lista_updateS {A} {AS : Setoid A} := injF3 (@lista_update A AS) _.
+
+Fixpoint lista_truncate0 {A} {AS : Setoid A} n  (a0 : A) (l : list A) :=
+  match n, l with
+    | 0, _ => []
+    | S n', [] => a0 :: lista_truncate0 n' a0 []
+    | S n', a' :: l' => a' :: lista_truncate0 n' a0 l'
+  end
+.
+
+Definition lista_truncate {A} {AS : Setoid A} n (a : A) (la : lista A) :=
+  match la with
+    | listaCons _ a0 l => listaCons _ a (lista_truncate0 n a0 l)
+  end
+.
+
+Instance lista_truncate_Proper A (AS : Setoid A): Proper (equiv ==> equiv ==> equiv ==> equiv) (@lista_truncate A AS).
+Proof.
+  autounfold. intros. rewrite H. clear x H. destruct x1, y1. generalize y H1. clear y H1. apply list_ind_2 with (l1:=l) (l2:=l0).
+  intros. simpl in H1. induction y.
+  simpl. tauto.
+  simpl. tauto. 
+  intros. destruct y.
+  simpl in *. split. eauto using lista_equiv0_equiv. auto.
+  simpl in *. split. symmetry.  tauto. apply H. tauto.
+  intros. destruct y.
+  simpl in *. split. eauto using lista_equiv0_equiv. auto.
+  simpl in *. split. tauto. apply H. tauto. 
+  intros. destruct y.
+  simpl in *. split. eauto using lista_equiv0_equiv. auto.
+  simpl in *. split. tauto. apply H. tauto.
+Qed.
+
+Definition lista_truncateS {A} {AS : Setoid A} := injF3 (@lista_truncate A AS) _.
+
+Lemma lista_equiv_lista_truncate: forall A (AS : Setoid A) n (a1 a2:A) (l1 l2 :lista A),
+                                       lista_truncate n a1 l1 == lista_truncate n a1 l2 ->
+                                       lista_truncate n a2 l1 == lista_truncate n a2 l2.
+Proof.
+  destruct l1, l2. generalize l l0. clear l l0. induction n.
+  simpl. intros. split. reflexivity. auto.
+  intros. destruct l, l0.
+  simpl in *. split. tauto. apply IHn. tauto.
+  simpl in *. split. tauto. apply IHn. tauto.
+  simpl in *. split. tauto. apply IHn. tauto.
+  simpl in *. split. tauto. apply IHn. tauto.
+Qed.
+
+Lemma lista_truncate_lista_update  :
+  forall {A} {AS : Setoid A} n (a : A)(a0:A )(n0:nat) (l1 l2:lista A),
+    lista_truncate n a l1 == lista_truncate n a l2 ->
+    lista_truncate n a (lista_updateS @ n0 @ l1 @ a0) == lista_truncate n a (lista_updateS @ n0 @ l2 @ a0).
+Proof.
+  destruct l1, l2. generalize n n0. clear n n0. apply list_ind_2 with (l1:=l) (l2:=l0).
+  intros. destruct n.
+  simpl. auto.
+  destruct H. rewrite H. reflexivity. 
+  intros. destruct n.
+  simpl. auto.
+  destruct H0. destruct n0.
+  simpl. split. reflexivity. auto.
+  simpl. split. auto. apply H. auto.
+  intros. destruct n.
+  simpl. auto.
+  destruct H0. destruct n0.
+  simpl.  split. reflexivity. auto.
+  simpl. split. auto. apply H. auto.
+  intros. destruct n.
+  simpl. auto.
+  destruct H0. destruct n0.
+  simpl. split. reflexivity. auto.
+  simpl. split. auto. apply H. auto.
+Qed.
+
+Fixpoint lista_zipWith0_right {A : Type} {AS : Setoid A} {B : Type} {BS : Setoid B} (f : AS ~> BS ~~> AS) (a : A)  (lb : list B) :=
+  match lb with
+    | [] => []
+    | b' :: lb' => (f @ a @ b') :: lista_zipWith0_right f a lb'
+  end
+.
+
+Fixpoint lista_zipWith0 {A : Type} {AS : Setoid A} {B : Type} {BS : Setoid B} (f : AS ~> BS ~~> AS) (a : A) (la : list A) (b : B) (lb : list B) :=
+  match la, lb with
+    | [] , _ => lista_zipWith0_right f a lb
+    | a' :: la', [] => (f @ a' @ b) :: lista_zipWith0 f a la' b []
+    | a' :: la', b' :: lb' => (f @ a' @ b') :: lista_zipWith0 f a la' b lb'
+  end
+.
+Definition lista_zipWith {A : Type} {AS : Setoid A} {B : Type} {BS : Setoid B} (f : AS ~> BS ~~> AS) (la : lista A) (lb : lista B) :=
+  match la, lb with
+    | listaCons _ a la' , listaCons _ b lb' => listaCons _ (f @ a @ b) (lista_zipWith0 f a la' b lb')
+  end
+.
+
+
+Instance lista_zipWith_Proper {A : Type} {AS : Setoid A}{B : Type} {BS : Setoid B} : Proper (equiv ==> equiv ==> equiv ==> equiv) (@lista_zipWith A _ B _).
+Proof.
+  autounfold. intros. destruct x0,y0,x1,y1. generalize H0 l1 l2 H1. clear H0 l1 l2 H1. apply list_ind_2 with (l1:=l) (l2:=l0).
+  - intros. destruct H0. unfold lista_zipWith.   simpl. generalize H1. clear H1. apply list_ind_2 with (l1:=l1) (l2:=l2).
+    + simpl. split. destruct H1. rewritesr. auto.
+    + intros. simpl in H1, H3. split. tauto. split.  destruct H3 as [? [? ?]]. rewritesr. tauto.
+    + intros. simpl in H1, H3. split. destruct H3. rewritesr. tauto.
+    + intros. simpl in H1, H3. split. destruct H3. rewritesr. tauto.
+  - intros. destruct l1, l2.
+    + simpl in H0, H1, H2. destruct H1 as [? [? ?]]. destruct H2. split. rewritesr. split. rewritesr. clear l l0 a1 H0 H1 H3 H5. induction b1.
+      * auto.
+      * simpl. destruct H4. split. rewritesr. apply IHb1. auto.
+    + simpl in H0, H1, H2. destruct H1 as [? [? ?]], H2 as [? [? ?]]. split. rewritesr. split. rewritesr. clear l l0 a1 H0 H3 H5. generalize H4 H6. clear H4 H6. apply list_ind_2' with (l1:=b1) (l2:=l2).
+      * simpl.  auto.
+      * intros. destruct H6. split. rewritesr. auto.
+      * intros. destruct H4. split. rewritesr. auto.
+      * intros. destruct H4, H6. split. rewritesr. auto.
+    + simpl in H0, H1, H2. destruct H1 as [? [? ?]], H2. split. rewritesr. apply H0. tauto. auto. 
+    + simpl in H0, H1, H2. destruct H1 as [? [? ?]], H2. split. rewritesr. apply H0. tauto. auto.
+  - intros. destruct l1, l2.
+    + simpl in H0, H1, H2. destruct H1, H2. split. rewritesr. apply (H0 H3 [] []). simpl. auto. 
+    + simpl in H0, H1, H2. destruct H1, H2 as [? [? ?]]. split. rewritesr. apply H0. auto. simpl. auto. 
+    + simpl in H0, H1, H2. destruct H1, H2. split. rewritesr. apply (H0 H3 l1 []). auto. 
+    + simpl in H0, H1, H2. destruct H1, H2. split. rewritesr. apply H0. auto. auto.
+  - intros. destruct l1, l2.
+    + simpl in H0, H1, H2. destruct H1, H2. split. rewritesr. apply H0. auto. simpl. auto. 
+    + simpl in H0, H1, H2. destruct H1, H2 as [? [? ?]]. split. rewritesr. apply H0. auto. simpl. auto.
+    + simpl in H0, H1, H2. destruct H1, H2. split. rewritesr. apply H0. auto.  auto.
+    + simpl in H0, H1, H2. destruct H1, H2. split. rewritesr. apply H0. auto. auto.
+Qed.
+
+
+Definition lista_zipWithS {A : Type} {AS : Setoid A} {B : Type} {BS : Setoid B} := injF3 (@lista_zipWith A _ B _) _.
+
+
+Definition lista_map  {A : Type} {AS : Setoid A} {B : Type} {BS : Setoid B} (f : AS ~> BS) (la : lista A) :=
+  match la with
+    | listaCons _ a la' => listaCons _ (f @ a) (mapS @ f @ la')
+  end
+.
+
+Instance lista_map_Proper {A : Type} {AS : Setoid A}{B : Type} {BS : Setoid B} : Proper (equiv ==> equiv ==> equiv) (@lista_map A _ B _).
+Proof.
+  autounfold. intros. destruct x0,y0. unfold lista_map.  rewrite H. clear x H.  generalize H0 . clear H0 . apply list_ind_2 with (l1:=l) (l2:=l0).
+  - intros. destruct H0. rewritesr.
+  - intros. destruct H0, H1. split. rewritesr. split. rewritesr. simpl in H. apply H. tauto.
+  - intros. destruct H0. split. rewritesr. simpl in H. apply H. auto. 
+  - intros. destruct H0. split. rewritesr. simpl in H. apply H. auto.  
+Qed.
+
+Definition lista_mapS  {A : Type} {AS : Setoid A}{B : Type} {BS : Setoid B}:= injF2 (@lista_map A AS B BS) _.
+
+Definition lista_nth {A : Type} {AS : Setoid A} n (l : lista A) :=
+  match l with
+    | listaCons _ a l' => nth n l' a
+  end
+.
+Instance lista_nth_Proper {A : Type} {AS : Setoid A} : Proper (equiv ==> equiv ==> equiv) lista_nth.
+Proof.
+  autounfold. intros. destruct x0, y0. simpl. rewrite H. clear x H. generalize y H0. clear y H0. apply list_ind_2 with (l1:=l) (l2:=l0).
+  - simpl. destruct y. tauto. tauto.
+  - intros.  destruct H0. destruct H1. simpl. destruct y. rewritesr. rewrite <- H. simpl. destruct y. reflexivity. reflexivity. simpl. auto.
+  - intros.  destruct H0. simpl. destruct y. rewritesr. rewrite H. simpl. destruct y. reflexivity. reflexivity. simpl. auto.
+  - intros.  destruct H0. simpl. destruct y. rewritesr. apply H. simpl.  auto.
+Qed.
+
+Definition lista_nthS {A : Type} {AS : Setoid A} := injF2 (@lista_nth A AS) _.
+
+Definition _listaNthLens' {A : Type} {AS : Setoid A} (n : nat) : _Lens' (lista A) A.
+  unfold _Lens'. intros. refine (lista_updateS @ n @ X0 <$> (X @ (lista_nthS @ n @ X0))).
+Defined.
+
+Definition _listaNthLens {f fS} {func : @Functor f fS} {A : Type} {AS : Setoid A} (n : nat) :=
+  @_listaNthLens' A AS n f fS func.
+
+Instance _listaNthLens_Proper {f fS} {func : @Functor f fS} {A : Type} {AS : Setoid A}(n : nat): Proper (equiv ==> equiv ==> equiv ) (@_listaNthLens f fS func A AS n).
+Proof.
+  autounfold. intros. unfold _listaNthLens, _listaNthLens'. rewritesr.
+Qed.
+
+Definition listaNthLens {f fS} {func : @Functor f fS} {A} {AS : Setoid A} (n : nat) :=
+  injF2 (@_listaNthLens f fS func A AS n) _.
+
+Fixpoint list_findn {A : Type} {AS : Setoid A} (p : AS ~> boolS) (a : A) (l : list A)  (n : nat) : maybe nat :=
+  match l with
+    | [] => if p @ a then Some n else None
+    | a' :: l' => if p @ a' then Some n else list_findn p a l' (S n)
+  end
+.
+
+Definition lista_find {A : Type} {AS : Setoid A} (p : AS ~> boolS) (l : lista A) : maybe nat :=
+  match l with
+    | listaCons _ a' l' => list_findn p a' l' 0
+  end
+.
+
+Instance lista_find_Proper {A : Type} {AS : Setoid A}: Proper (equiv ==> equiv ==> equiv ) (@lista_find A AS).
+Proof.
+  autounfold. intros. destruct x0, y0.  unfold lista_find. generalize 0 H0. clear H0. apply list_ind_2 with (l1:=l) (l2:=l0).
+  - intros. destruct H0.  match goal with
+      | |- ?a == ?b => simpl a; simpl b
+    end. matchequiv.  inversion H2. inversion H2. 
+  - intros. destruct H1 as [? [? ?]].
+    match goal with
+      | |- ?a == ?b => simpl a; simpl b
+    end. rewrite H , H2. assert (y @ a = true \/ y @ a = false). destruct (y @ a). tauto. tauto. destruct H4. rewrite H4. reflexivity.  rewrite H4. rewrite <- H0. simpl. rewrite <- H in H4. rewrite H4. auto. simpl.   auto.
+  - intros. destruct H1 as [? ?].
+    match goal with
+      | |- ?a == ?b => simpl a; simpl b
+    end. rewrite H , H1. assert (y @ a0 = true \/ y @ a0 = false). destruct (y @ a0). tauto. tauto. destruct H3. rewrite H3. reflexivity.  rewrite H3. rewrite H0. simpl. rewrite H3. auto. simpl.   auto.
+  - intros. destruct H1 as [? ?].
+    match goal with
+      | |- ?a == ?b => simpl a; simpl b
+    end. rewrite H , H1. assert (y @ c = true \/ y @ c = false). destruct (y @ c). tauto. tauto. destruct H3. rewrite H3. reflexivity.  rewrite H3. apply H0. auto. 
+Qed.
+
+Definition lista_findS {A} {AS : Setoid A} :=
+  injF2 (@lista_find A AS) _.
+
+
+Fixpoint list_findan {A : Type} {AS : Setoid A} (d : forall a a' : A, {a==a'} + {~a==a'}) (a : A) (l : list A)  (n : nat) :  nat :=
+  match l with
+    | [] =>  n
+    | a' :: l' => if d a a' then  n else list_findan d a l' (S n)
+  end
+.
+
+Definition lista_finda {A : Type} {AS : Setoid A} (d : forall a a' : A, {a==a'} + {~a==a'}) (l : lista A) :  nat :=
+  match l with
+    | listaCons _ a' l' => list_findan d a' l' 0
+  end
+.
+
+Instance lista_finda_Proper {A : Type} {AS : Setoid A} d: Proper (equiv ==> equiv ) (@lista_finda A AS d).
+Proof.
+  autounfold. intros. destruct x, y.  unfold lista_finda. generalize 0 H. clear H. apply list_ind_2 with (l1:=l) (l2:=l0).
+  - intros. simpl. auto. 
+  - intros. destruct H0 as [? [? ?]].
+    simpl. destruct (d a0 a1). reflexivity.  rewrite H1 in n0. symmetry in H0. tauto.
+    
+  - intros. destruct H0 as [? ?].
+    simpl. destruct (d a a1). reflexivity.  pose (listaCons_equiv _ _ a a0 b [] H1). rewrite H0 in n0. tauto.
+  - intros. destruct H0 as [? ?].
+    match goal with
+      | |- ?a == ?b => simpl a; simpl b
+    end. pose (listaCons_equiv _ _ a a0 b d0 H1). destruct (d a a1), (d a0 c). reflexivity. rewrite <- e, <- H0 in n0. tauto. rewrite <- e, <- H0 in e0. tauto. apply H. auto. 
+Qed.
+
+Definition lista_findaS {A} {AS : Setoid A} d :=
+  injF (@lista_finda A AS d) _.
+
+Definition lista_repeat {A : Type} {AS : Setoid A} (a : A) := listaCons _ a [].
+Instance lista_repeat_Proper {A : Type} {AS : Setoid A} : Proper (equiv ==> equiv ) (@lista_repeat A AS).
+Proof.
+  autounfold. intros. simpl. auto.
+Qed.
+
+Definition lista_repeatS {A : Type} {AS : Setoid A} := injF (@lista_repeat A AS) _.
+
+Fixpoint list_filter_index {A : Type} {AS : Setoid A} (p : AS ~> boolS) (l : list A) n : list nat :=
+  match l with
+    | [] => []
+    | a' :: l' => if p @ a' then n :: list_filter_index p l' (S n) else list_filter_index p l' (S n)
+  end
+.
+
+Definition lista_filter_index {A : Type} {AS : Setoid A} (p : AS ~> boolS) (l : lista A) : list nat :=
+  match l with
+    | listaCons _ a' l' => if (p @ a') then [] else list_filter_index p l' 0
+  end
+.
+
+Instance lista_filter_index_Proper {A : Type} {AS : Setoid A}: Proper (equiv ==> equiv ==> equiv ) (@lista_filter_index A AS).
+Proof.
+  autounfold. intros. destruct x0, y0.  unfold lista_filter_index. generalize 0 H0. clear H0. apply list_ind_2 with (l1:=l) (l2:=l0).
+  - intros. destruct H0. simpl. matchequiv.  
+  - intros. destruct H1 as [? [? ?]].
+    match goal with
+      | |- ?a == ?b => simpl a; simpl b
+    end. rewrite H , <- H1, H2. assert (y @ a = true \/ y @ a = false). destruct (y @ a). tauto. tauto. destruct H4. rewrite H4. reflexivity.  rewrite H4. rewrite <- H in H4. rewrite H4 in H0. rewrite H, H1 in H4. rewrite H4 in H0. rewrite <- H0. simpl. auto.  simpl.   auto.
+  - intros. destruct H1 as [? ?].
+    match goal with
+      | |- ?a == ?b => simpl a; simpl b
+    end.  pose (listaCons_equiv _ _ a a0 b [] H2).   assert (x @ a = true \/ x @ a = false). destruct (x @ a). tauto. tauto. destruct H3. rewrite H3. rewrite H, e in H3. rewrite H3. reflexivity.  rewrite H3. rewrite e, <- H1 in H3. rewrite H3. rewrite H1 , <- e in H3. rewrite H3 in H0. rewrite H, e in H3. rewrite H3 in H0. rewrite H0. simpl. rewrite H3. auto. simpl.   auto.
+  - intros. destruct H1 as [? ?].
+    match goal with
+      | |- ?a == ?b => simpl a; simpl b
+    end.  pose (listaCons_equiv _ _ a a0 b d H2). assert (x @ a = true \/ x @ a = false). destruct (x @ a). tauto. tauto. destruct H3. rewrite H3 in *. rewrite H, e in H3. rewrite H3 in *. auto.   rewrite H3 in *. rewrite H, H1. rewrite H, e in H3. rewrite H3 in *. destruct (y @ c). constructor. reflexivity. apply H0. auto.  apply H0. auto.
+Qed.
+
+Definition lista_filter_indexS {A} {AS : Setoid A} :=
+  injF2 (@lista_filter_index A AS) _.
+
+Fixpoint list_filter_index' {A : Type} {AS : Setoid A}  (l : list (maybe A)) n : list (nat * A) :=
+  match l with
+    | [] => []
+    | a' :: l' =>
+      match a' with
+        | Some a' => (n, a') :: list_filter_index'  l' (S n)
+        | None => list_filter_index'  l' (S n)
+      end
+  end
+.
+
+Definition lista_filter_index' {A : Type} {AS : Setoid A}  (l : lista (maybe A)) : list (nat * A) :=
+  match l with
+    | listaCons _ a' l' =>
+      match a' with
+        | Some _ =>  []
+        | None => list_filter_index' l' 0
+      end
+  end
+.
+
+Instance lista_filter_index'_Proper {A : Type} {AS : Setoid A}: Proper (equiv ==> equiv ) (@lista_filter_index' A AS).
+Proof.
+  autounfold. intros. destruct x, y.  unfold lista_filter_index'. generalize 0 H. clear H. apply list_ind_2 with (l1:=l) (l2:=l0).
+  - intros. destruct H. simpl. matchequiv.  
+  - intros. destruct H0 as [? [? ?]]. matchequiv.  destruct a. inversion H1. simpl. rewrite <- H. reflexivity. simpl.  auto. 
+  - intros. destruct H0.  pose (listaCons_equiv _ _ m m0 b [] H1). matchequiv. destruct a.  inversion H0. simpl.  rewrite H. simpl. reflexivity.   simpl.   auto.
+  - intros. destruct H0.  pose (listaCons_equiv _ _ m m0 b d H1). matchequiv. simpl. matchequiv. constructor. simpl in H3. rewritesr. apply H. auto. apply H. auto.
+Qed.
+
+Definition lista_filter_indexS' {A} {AS : Setoid A} :=
+  injF (@lista_filter_index' A AS) _.
+
+(* partial matrix *)
+
+Inductive matrixp A {AP : Pointed A} : Type := matrixpCons : nat -> lista (option (lista A)) -> matrixp A. 
+
+
+Existing Instance maybe_Monad.
+Existing Instance monadFunctor.
+Definition _rows  {A : Type} {AS : Setoid A} {AP : Pointed A} (mat : matrixp A) : lista (maybe (lista A)) := match mat with
+                     | matrixpCons _ w rows => lista_mapS @ (fmap @ (lista_truncateS @ w @ point)) @ rows
+                   end.
+
+
+Definition matrixp_equiv {A} {AS : Setoid A}{AP : Pointed A} (m1 m2 : matrixp A) : Prop :=
+  match m1, m2 with
+    | matrixpCons _ n l, matrixpCons _ n0 l0 =>
+      n = n0 /\ _rows m1 == _rows m2
+  end.
+
+
+Hint Unfold matrixp_equiv.
+
+Instance matrixp_equiv_Equivalence {A} {AS : Setoid A} {AP : Pointed A}: Equivalence (matrixp_equiv).
+Proof.
+  split.
+  - autounfold. intros. destruct x. split. auto. reflexivity. 
+  - autounfold. intros. destruct x, y. destruct H. split. auto. symmetry. auto. 
+  - autounfold. intros. destruct x, y, z. destruct H, H0. split. congruence. transitivity (_rows (matrixpCons A n0 l0)). auto.
+auto.
+Qed.
+
+
+Instance matrixpS {A} (AS : Setoid A) {AP : Pointed A} : Setoid (matrixp A) :=
+  {
+    equiv := matrixp_equiv
+  }
+.
+
+Instance _rows_Proper A (AS : Setoid A) (AP : Pointed A) : Proper (equiv ==> equiv) (@_rows A AS AP).
+Proof.
+  autounfold. intros. destruct x, y, l, l0. unfold _rows. inversion H. clear H. rewrite H0 in *. clear n H0. generalize H1. clear H1. apply list_ind_2 with (l1:= l) (l2:=l0).
+  - intros. auto.  
+  - intros. destruct H1. destruct H1. split. auto. split. auto. apply H. split. auto. auto.
+  - intros. destruct H1. split. auto. apply H. auto.
+  - intros. destruct H1. split. auto. apply H. auto.
+Qed.
+
+Definition rows {A : Type} {AS : Setoid A} {AP : Pointed A} := injF (@_rows A AS AP) _.
+
+Lemma lista_truncate_equiv_equiv : forall A (AS : Setoid A) l1 l2 n (a : A),  l1 == l2 -> lista_truncate n a l1 == lista_truncate n a l2.
+Proof.
+  intros. generalize n H. clear n H . destruct l1, l2. apply list_ind_2 with (l1:=l) (l2:=l0).
+  - simpl. intros. induction n.
+    + simpl. split. reflexivity. auto.
+    + simpl. tauto.
+  - intros. destruct H0.  destruct H1. induction n.
+    + simpl. split. reflexivity. auto.
+    + simpl. split. symmetry. auto. apply H. simpl. auto. 
+  - intros. destruct H0.  induction n.
+    + simpl. split. reflexivity. auto.
+    + simpl. split. auto. apply H. simpl. auto. 
+  - intros. destruct H0.  induction n.
+    + simpl. split. reflexivity. auto.
+    + simpl. split. auto. apply H. simpl. auto. 
+Qed.
+
+Instance matrixpCons_Proper {A : Type} {AS : Setoid A} {AP : Pointed A} : Proper (equiv ==> equiv ==> equiv) (@matrixpCons A AP).
+Proof.
+  autounfold. intros. split. auto. destruct x0, y0. destruct o, o0.
+  - generalize H0. clear H0. apply list_ind_2 with (l1:=l) (l2:=l0).
+    + intros. destruct H0. split. rewritesr. auto. 
+    + intros. destruct H1. destruct H2. split. apply H0. simpl.  auto. split. rewritesr. apply H0. simpl. auto. 
+    + intros. destruct H1. split. rewritesr. apply H0. simpl. auto.
+    + intros. destruct H1. split. rewritesr. apply H0. simpl. auto.
+  - pose (listaCons_equiv _ _ (Some l1) None l l0 H0). inversion e. 
+  - pose (listaCons_equiv _ _ None (Some l1)  l l0 H0). inversion e. 
+  - generalize H0. clear H0. apply list_ind_2 with (l1:=l) (l2:=l0).
+    + intros. destruct H0. split. rewritesr. auto.
+    + intros. destruct H1. destruct H2. split. apply H0. simpl.  auto. split. rewritesr. apply H0. simpl. auto. 
+    + intros. destruct H1. split. rewritesr. apply H0. simpl. auto.
+    + intros. destruct H1. split. rewritesr. apply H0. simpl. auto.
+Qed.
+
+(* read matrix column *)
+
+
+Definition _readCol {A : Type} {AS : Setoid A} (w n : nat) (l : maybe (lista A)) :=
+  if lt_dec n w then
+    match l with
+      | None => None
+      | Some l' => Some (lista_nth n l')
+    end
+  else
+    None.
+Lemma _readCol_lista_truncate :
+  forall {A : Type} {AS : Setoid A} (w n : nat) (a : A) (l :  lista A),
+    _readCol w n (Some l) == _readCol w n (Some (lista_truncate w a l)).
+
+Proof.
+
+  intros. destruct l. unfold _readCol. destruct (lt_dec n w).
+  - simpl. generalize w l0 l. clear w l0 l. induction n.
+    + intros.  destruct w.
+      * inversion l0.
+      * destruct l. simpl. reflexivity. simpl. reflexivity. 
+    +  intros. destruct w.
+       * inversion l0.
+       * destruct l. simpl. rewrite <- IHn. simpl. destruct n. reflexivity. reflexivity.
+    apply le_S_n. auto.
+    simpl. rewrite <- IHn. reflexivity. apply le_S_n.  auto.
+  - reflexivity.
+Qed.
+  
+Instance _readCol_Proper {A : Type} {AS : Setoid A} : Proper (equiv ==> equiv ==> equiv ==> equiv) (@_readCol A AS).
+Proof.
+  autounfold. intros. unfold _readCol. simpl in H, H0. rewrite H, H0. destruct (lt_dec y0 y). matchequiv. destruct l0, l1.  simpl in H1. simpl. clear x H x0 H0. generalize y0 H1 l. clear y0 H1 l. apply list_ind_2 with (l1:=l0)(l2:=l1).
+  intros. simpl in *.  destruct y0. tauto. tauto.
+  intros. destruct y0. simpl in *. symmetry. tauto. simpl. rewrite <- H. destruct y0.  reflexivity. reflexivity. simpl in *. tauto. apply Nat.lt_le_incl. auto. 
+  intros. destruct y0. simpl in *. tauto. simpl. rewrite H. destruct y0.  reflexivity. reflexivity. simpl in *. tauto. apply Nat.lt_le_incl. auto. 
+  intros. destruct y0. simpl in *. tauto. simpl. apply H. simpl in *. tauto. apply Nat.lt_le_incl. auto.
+  reflexivity. 
+Qed.
+
+Definition readCol {A : Type} {AS : Setoid A} := injF3 (@_readCol A AS) _. 
+
+Definition readWholeCol {A} {AS : Setoid A} w n := lista_mapS @ (readCol @ w @ n).
+
+Definition _readMatrixCol {A : Type} {AS : Setoid A} {AP : Pointed A} n mat :=
+  match mat with
+    | matrixpCons _ w l => readWholeCol w n @ l
+  end.
+Lemma lista_nth_truncate_equiv : forall A (AS:Setoid A) n0 (a :A) (l1 l2 : lista A) n, lista_truncate n0 a l1 == lista_truncate n0 a l2 -> n < n0 -> lista_nth n l1 == lista_nth n l2.
+Proof.
+  intros. destruct l1, l2. generalize n n0 H0 H.  clear n n0 H0 H. apply list_ind_2 with (l1:=l) (l2:=l0).
+  - simpl. intros. destruct n0. inversion H0. destruct H. destruct n. auto.  auto.
+  - intros. simpl in *. destruct n0.  inversion H0. destruct H1. destruct n. auto. rewrite <- H with (n0 := n0). destruct n. reflexivity. reflexivity. apply le_S_n. auto. auto.
+  - intros. simpl in *. destruct n0.  inversion H0. destruct H1. destruct n. auto. rewrite H with (n0 := n0). destruct n. reflexivity. reflexivity. apply le_S_n. auto. auto.
+  - intros. simpl in *. destruct n0.  inversion H0. destruct H1. destruct n. auto. apply H with (n0 := n0). apply le_S_n. auto. auto.
+Qed.
+
+Lemma readCol_truncate_equiv : forall A (AS:Setoid A) (w n : nat) a (l1 l2 : lista A) n, lista_truncate w a l1 == lista_truncate w a l2 -> readCol @ w @ n @ Some l1 == readCol @ w @ n @ Some l2.
+Proof.
+  intros. simpl. unfold _readCol. destruct (lt_dec n0 w). apply (lista_nth_truncate_equiv _ _ w a). auto. auto. auto.
+Qed.
+
+Instance _readMatrixCol_Proper {A} {AS : Setoid A} {AP : Pointed A} : Proper (equiv ==> equiv ==> equiv) (@_readMatrixCol A AS AP).
+Proof.
+  autounfold. intros. destruct x0, y0. unfold _readMatrixCol. rewrite H. clear x H. destruct H0.  rewrite H in *. clear n H. generalize H0. clear H0. destruct l, l0. destruct o, o0.
+  - apply list_ind_2 with (l1:=l)(l2:=l0).
+    + intros. destruct H0. simpl in H, H0.   split. apply (readCol_truncate_equiv _ _ n0 y point). auto. auto. 
+    + intros. destruct H0. destruct H1. destruct a.
+      * split. apply (readCol_truncate_equiv _ _ n0 y point). auto. split. apply (readCol_truncate_equiv _ _ n0 y point). auto. apply H.  split. auto. auto.
+      * inversion H1.
+    + intros. destruct H0. destruct a.
+      * split. apply (readCol_truncate_equiv _ _ n0 y point). auto. apply H.  auto. 
+      * inversion H0.
+    + intros. destruct H0. destruct a, c.
+      * split. apply (readCol_truncate_equiv _ _ n0 y point). auto. apply H.  auto. 
+      * inversion H0.
+      * inversion H0.
+      * split. reflexivity. apply H. auto.
+        
+  - intros. generalize H0. clear H0. apply list_ind_2 with (l1:=l)(l2:=l0).
+    + intros. destruct H0. inversion H. 
+    + intros. destruct H0. inversion H0.
+    + intros. destruct H0. destruct a.
+      * inversion H0.
+      * split. reflexivity. apply H. auto.
+    + intros. destruct H0. destruct a, c.
+      * split. apply (readCol_truncate_equiv _ _ n0 y point). auto. apply H.  auto. 
+      * inversion H0.
+      * inversion H0.
+      * split. reflexivity. apply H. auto.
+  - intros. generalize H0. clear H0. apply list_ind_2 with (l1:=l)(l2:=l0).
+    + intros. destruct H0. inversion H. 
+    + intros. destruct H0. inversion H0.
+    + intros. destruct H0. destruct a.
+      * split. apply (readCol_truncate_equiv _ _ n0 y point). auto. apply H. auto.
+      * inversion H0.
+    + intros. destruct H0. destruct a, c.
+      * split. apply (readCol_truncate_equiv _ _ n0 y point). auto. apply H.  auto. 
+      * inversion H0.
+      * inversion H0.
+      * split. reflexivity. apply H. auto.
+  - apply list_ind_2 with (l1:=l)(l2:=l0).
+    + intros. destruct H0. simpl in H, H0.   split. reflexivity. auto. 
+    + intros. destruct H0. destruct H1. destruct a.
+      * inversion H1.
+      * split. reflexivity. split.  reflexivity.  apply H. split.  auto.  auto. 
+    + intros. destruct H0. destruct a.
+      * inversion H0.
+      * split. reflexivity. apply H. auto. 
+    + intros. destruct H0. destruct a, c.
+      * split. apply (readCol_truncate_equiv _ _ n0 y point). auto. apply H.  auto. 
+      * inversion H0.
+      * inversion H0.
+      * split. reflexivity. apply H. auto.
+Qed.
+
+Definition readMatrixCol {A : Type} {AS : Setoid A}{AP: Pointed A} := injF2 (@_readMatrixCol A AS AP) _.
+
+Definition _updateCol {A : Type} {AS : Setoid A} n (l: maybe (lista A)) (a : maybe A) :=
+  match l, a with
+    | None, _ => None
+    | _, None => l
+    | Some l', Some a' => Some (lista_updateS @ n @ l' @ a')
+  end
+.
+
+Instance _updateCol_Proper {A : Type} {AS : Setoid A} : Proper (equiv ==> equiv ==> equiv ==> equiv) (@_updateCol A AS).
+Proof.
+  autounfold. intros. destruct x0, y0, x1, y1. simpl. simpl in H0, H1. rewrite H, H0, H1. reflexivity. 
+  inversion H1.
+  inversion H1.
+  simpl. auto.
+  inversion H0.
+  inversion H0.
+  inversion H0.
+  inversion H0.
+  inversion H0.
+  inversion H0.
+  inversion H0.
+  inversion H0.
+  simpl. auto.
+  inversion H1.
+  inversion H1.
+  simpl. auto.
+Qed.
+
+Definition updateCol {A : Type} {AS : Setoid A} := injF3 (@_updateCol A AS) _.
+
+Definition updateWholeCol {A : Type} {AS : Setoid A} n : listaS (maybeS (listaS AS)) ~> listaS (maybeS AS) ~~> listaS (maybeS (listaS AS)) :=
+  lista_zipWithS @ (updateCol @ n).
+
+
+
+Definition _updateMatrixCol {A : Type} {AS : Setoid A} {AP : Pointed A} n mat col  :=
+  match mat with
+    | matrixpCons _ w l => matrixpCons _ w (updateWholeCol n @ l @ col)
+  end.
+
+Hint Unfold _updateMatrixCol.
+
+
+(*Lemma matrixp_equiv_cons : forall {A : Type} {AS : Setoid A} w (a1 a2 : A) (a b : maybe (list A)) (la lb : list (maybe (list A))), matrixp_equiv0 w (a::la) (b::lb) = lista_equiv w (listaCons a1 a) (listaCons a2 b) /\ matrixp_equiv0 w a1 a2 la lb.
+
+Proof.
+  intros. reflexivity.
+Qed.*)
+
+
+Instance _updateMatrixCol_Proper {A} {AS : Setoid A} {AP : Pointed A} : Proper (equiv ==> equiv ==> equiv ==> equiv) (@_updateMatrixCol A AS AP).
+Proof.
+  autounfold. intros. destruct x0, y0. destruct x1, y1.  destruct l, l0. destruct  H0.   rewrite H, H0, H1 in *.  clear H0 H H1. generalize H2. clear H2. apply (list_ind_3') with (l1:=l) (l2:=l0) (l3:=l2).
+  - split. auto. split.
+    + destruct o1, o2, o0.
+      * simpl. simpl in H2. apply lista_truncate_lista_update. tauto.
+      * simpl. simpl in H2. tauto.
+      * simpl. simpl in H2.  tauto.
+      * simpl. simpl in H2. tauto.
+      * simpl. simpl in H2. tauto.
+      * simpl. simpl in H2. tauto.
+      * simpl. auto.
+      * simpl. auto.
+    + simpl. auto. 
+  - split. auto. split. destruct H2.
+    + destruct o1, o2, a. 
+      * simpl. simpl in H0. apply lista_truncate_lista_update. auto.
+      * simpl. simpl in H0. auto.
+      * simpl in H0.  tauto.
+      * simpl in H0. tauto.
+      * simpl in H0. tauto.
+      * simpl in H0. tauto.
+      * simpl. auto.
+      * simpl. auto.
+    + apply H. auto.
+  - split. auto. split. destruct H2.
+    + destruct o1, o2, o0. 
+      * simpl. simpl in H0. apply lista_truncate_lista_update. auto.
+      * simpl. simpl in H0. auto.
+      * simpl in H0.  tauto.
+      * simpl in H0. tauto.
+      * simpl in H0. tauto.
+      * simpl in H0. tauto.
+      * simpl. auto.
+      * simpl. auto.
+    + split. destruct H2. destruct H1. destruct a, o1, o0. 
+      * simpl. simpl in H1. apply lista_truncate_lista_update. auto.
+      * simpl. simpl in H1. auto.
+      * simpl in H1.  tauto.
+      * simpl in H1. tauto.
+      * simpl in H1. tauto.
+      * simpl in H1. tauto.
+      * simpl. auto.
+      * simpl. auto.
+    * apply H.  destruct H2.  destruct H1. split.  auto. auto.
+  - split. auto. split. destruct H2. destruct H1.
+    + destruct o1, a, c. 
+      * simpl. simpl in H1. symmetry. apply lista_truncate_lista_update. auto.
+      * simpl. simpl in H1. symmetry. auto.
+      * simpl in H1.  tauto.
+      * simpl in H1. tauto.
+      * simpl in H1. tauto.
+      * simpl in H1. tauto.
+      * simpl. auto.
+      * simpl. auto.
+    + apply H.  destruct H2.  destruct H1. split.  auto. auto.
+  - split. auto. split. destruct H2.
+    + destruct a, o2, o0. 
+      * simpl. simpl in H0. apply lista_truncate_lista_update. auto.
+      * simpl. simpl in H0. auto.
+      * simpl in H0.  tauto.
+      * simpl in H0. tauto.
+      * simpl in H0. tauto.
+      * simpl in H0. tauto.
+      * simpl. auto.
+      * simpl. auto.
+    + apply H.  destruct H2.  auto.
+  - split. auto. split. destruct H2.
+    + destruct a, o2, c. 
+      * simpl. simpl in H0. apply lista_truncate_lista_update. auto.
+      * simpl. simpl in H0. auto.
+      * simpl in H0.  tauto.
+      * simpl in H0. tauto.
+      * simpl in H0. tauto.
+      * simpl in H0. tauto.
+      * simpl. auto.
+      * simpl. auto.
+    + apply H.  destruct H2.  auto.
+  - split. auto. split. destruct H2.
+    + destruct a, c, o0. 
+      * simpl. simpl in H0. apply lista_truncate_lista_update. auto.
+      * simpl. simpl in H0. auto.
+      * simpl in H0.  tauto.
+      * simpl in H0. tauto.
+      * simpl in H0. tauto.
+      * simpl in H0. tauto.
+      * simpl. auto.
+      * simpl. auto.
+    + apply H.  destruct H2.  auto.
+  - split. auto. split. destruct H2.
+    + destruct a, c, e. 
+      * simpl. simpl in H0. apply lista_truncate_lista_update. auto.
+      * simpl. simpl in H0. auto.
+      * simpl in H0.  tauto.
+      * simpl in H0. tauto.
+      * simpl in H0. tauto.
+      * simpl in H0. tauto.
+      * simpl. auto.
+      * simpl. auto.
+    + apply H.  destruct H2.  auto.
+Qed.
+
+Definition updateMatrixCol {A} {AS : Setoid A} {AP : Pointed A} := injF3 (@_updateMatrixCol A AS AP) _.
+
+Definition _matrixColLens' {A} {AS : Setoid A} {AP : Pointed A} (n : nat) : _Lens' (matrixp A) (lista (maybe A)).
+  unfold _Lens'. intros. refine (
+                              updateMatrixCol @ n @
+                                X0
+                                <$> (X @ (readMatrixCol @ n @ X0))).
+Defined.
+
+Definition _matrixColLens {f fS }{func : @Functor f fS} {A} {AS : Setoid A} {AP : Pointed A} (n : nat) :
+  (listaS (maybeS AS) ~> fS _ (listaS (maybeS AS))) -> matrixp A -> f (matrixp A) _ := _matrixColLens' n f fS func.
+
+Instance _matrixColLens_Proper {f fS} {func : @Functor f fS} A (AS : Setoid A) (AP : Pointed A) : Proper (equiv ==> equiv ==> equiv ==> equiv) (_matrixColLens).
+Proof.
+  autounfold. intros. unfold _matrixColLens, _matrixColLens'. rewritesr. 
+Qed.
+
+Definition matrixColLens {f fS} {func : @Functor f fS} {A} {AS : Setoid A} {AP : Pointed A} := injF3 _matrixColLens _.
+
+
+
+Definition _width  {A : Type} {AS : Setoid A} {AP : Pointed A} (mat : matrixp A) : nat.
+  simple refine (  match mat with
+                     | matrixpCons _ w _ => w
+                   end)
+.
+Defined.
+
+Instance _width_Proper A (AS : Setoid A) AP : Proper (equiv ==> equiv) (@_width A AS AP).
+Proof.
+  autounfold. intros. destruct x,y. destruct H. simpl. auto.
+Qed.
+
+Definition width {A : Type} {AS : Setoid A} {AP} := injF (@_width A AS AP) _.
+
+Definition matrixpConsS {A : Type} {AS : Setoid A} {AP : Pointed A} := injF2 (matrixpCons A) _.
+
+Definition _matrixWidthLens' {A : Type} {AS : Setoid A} {AP : Pointed A}  : _Lens' (matrixp A) nat.
+  unfold _Lens'. intros. refine (flipS @ matrixpConsS @ (rows @ X0) <$> (X @ (width @ X0))).
+Defined.
+
+Definition _matrixWidthLens {f fS} {func : @Functor f fS} {A : Type} {AS : Setoid A} {AP : Pointed A}  :=
+  @_matrixWidthLens' A AS AP f fS func.
+
+Instance _matrixWidthLens_Proper {f fS} {func : @Functor f fS} {A : Type} {AS : Setoid A}{AP: Pointed A}: Proper (equiv ==> equiv ==> equiv ) (@_matrixWidthLens f fS func A AS AP).
+Proof.
+  autounfold. intros. unfold _matrixWidthLens, _matrixWidthLens'. rewritesr.
+Qed.
+
+Definition matrixWidthLens {f fS} {func : @Functor f fS} {A} {AS : Setoid A} {AP: Pointed A} :=
+  injF2 (@_matrixWidthLens f fS func A AS AP ) _.
+
+Definition _matrixRowsLens' {A : Type} {AS : Setoid A} {AP : Pointed A}  : _Lens' (matrixp A) (lista (maybe (lista A))).
+  unfold _Lens'. intros. refine (matrixpConsS @ (width @ X0) <$> (X @ (rows @ X0))).
+Defined.
+
+Definition _matrixRowsLens {f fS} {func : @Functor f fS} {A : Type} {AS : Setoid A} {AP : Pointed A}  :=
+  @_matrixRowsLens' A AS AP f fS func.
+
+Instance _matrixRowsLens_Proper {f fS} {func : @Functor f fS} {A : Type} {AS : Setoid A} {AP : Pointed A} : Proper (equiv ==> equiv ==> equiv ) (@_matrixRowsLens f fS func A AS AP).
+Proof.
+  autounfold. intros. unfold _matrixRowsLens, _matrixRowsLens'. rewritesr.
+Qed.
+
+Definition matrixRowsLens {f fS} {func : @Functor f fS} {A} {AS : Setoid A} {AP : Pointed A}  :=
+  injF2 (@_matrixRowsLens f fS func A AS AP ) _.
+
+Require Import MaybeLens.
+Definition matrixRowTraversal {f fS func} {app : @Applicative f fS func} {A} {AS : Setoid A} {AP : Pointed A}(n : nat) :=
+  matrixRowsLens ∘ listaNthLens n ∘ maybePrism. 
+
+Definition matrixCellTraversal {f fS func} {app : @Applicative f fS func} {A} {AS : Setoid A} {AP:Pointed A}(m n : nat) :=
+  matrixRowTraversal m ∘ listaNthLens n.
+
