Algebra/Lens/MaybeLens.v
@@ -1,0 +1,26 @@
+Require Import Algebra.Functor Algebra.Applicative Algebra.SetoidCat Algebra.PairUtils Algebra.SetoidUtils Algebra.Monad Tactics Utils Algebra.Lens.LensTypes Algebra.Maybe.
+Require Import SetoidClass Vector.
+
+Instance Some_Proper A (AS : Setoid A) : Proper (equiv ==> equiv) (@Some A).
+Proof.
+  autounfold. intros. simpl. auto.
+Qed.
+
+Definition SomeS {A} {AS : Setoid A} : AS ~> maybeS AS := injF Some _.
+
+Definition _maybePrism' {A} {AS : Setoid A} : _Prism' (maybe A) A.
+  unfold _Prism'. intros. refine (match X0 with
+                                    | None => pure @ X0
+                                    | Some a => SomeS <$> X @ a
+                                  end).
+Defined.
+
+Definition _maybePrism {f fS func} {app : @Applicative f fS func} {A} {AS : Setoid A} :
+  (AS ~> fS _ AS) -> maybe A -> f (maybe A) _ := _maybePrism' f fS func app.
+
+Instance _maybePrism_Proper {f fS func} {app : @Applicative f fS func} A (AS : Setoid A) : Proper (equiv ==> equiv ==> equiv) (_maybePrism).
+Proof.
+  autounfold. intros. unfold _maybePrism, _maybePrism'. matchequiv. simpl in H0.  rewritesr.
+Qed.
+
+Definition maybePrism {f fS func} {app : @Applicative f fS func} {A} {AS : Setoid A} := injF2 _maybePrism _.
