Algebra/Pointed.v
@@ -1,0 +1,11 @@
+Class Pointed A : Type :=
+  {
+    point : A
+  }
+.
+
+
+Instance nat_Pointed : Pointed nat :=
+  {
+    point := 0
+  }.
