SQL/SQL.v
@@ -1,0 +1,315 @@
+Require Import Assert Command Definitions Algebra.Monoid Expr Algebra.SetoidCat Algebra.Maybe Tactics Algebra.ListUtils Algebra.Functor Algebra.Applicative Algebra.Alternative Algebra.FoldableFunctor Algebra.PairUtils Algebra.Maybe Algebra.Monad Algebra.Lens.Lens ListLens Utils SetoidUtils MonoidUtils Pointed.
+Require Import Coq.Structures.DecidableTypeEx List  SetoidClass PeanoNat FMapWeakList Basics Coq.Init.Specif.
+
+Module FMapNat := FMapWeakList.Make Nat_as_DT.
+Module NatNat_as_DT := PairDecidableType Nat_as_DT Nat_as_DT.
+Module FMapNatNat := FMapWeakList.Make NatNat_as_DT.
+
+Definition singleton {T} (k : nat) (v : T) : FMapNat.t T :=
+  FMapNat.add k v (FMapNat.empty T).
+
+
+Inductive sqlVal :=
+| vNat : nat -> sqlVal
+| vRow : list nat -> sqlVal
+.
+
+Program Instance sqlValS : Setoid sqlVal.
+
+Module SQLValType <: ValType.
+  Definition val := sqlVal.
+  Instance valS : Setoid sqlVal :=
+    {
+      equiv := eq
+    }.
+  Lemma equiv_dec : forall val1 val2, {val1 == val2} + {~ val1 == val2}.
+  Proof.
+    intros. simpl. destruct val1, val2. destruct (Nat.eq_dec n n0). left. congruence.
+    right. congruence.
+    right. intro. inversion H.
+    right. intro. inversion H.
+    destruct (list_eq_dec Nat.eq_dec l l0).
+    left. congruence.
+    right. congruence.
+  Qed.
+End SQLValType.
+
+Definition table := nat.
+Instance tableS : Setoid nat := natS.
+Definition colind := nat.
+Definition coltype := nat.
+Definition tableSchema := list coltype.
+Definition sqlBuiltIn := nat.
+
+
+Section SQLSyntax.
+  
+
+  Inductive sqlExpr :=
+  | sqlValExpr : sqlVal -> sqlExpr
+  | sqlVarExpr : var -> sqlExpr
+  | sqlAppExpr : sqlBuiltIn -> list sqlExpr -> sqlExpr
+  | sqlColExpr : sqlExpr -> colind -> sqlExpr
+  .
+
+  Program Instance sqlExprS : Setoid sqlExpr. 
+
+  Inductive sqlFormula :=
+  | sqlBuiltInFormula : sqlBuiltIn -> list sqlExpr -> sqlFormula
+  | sqlAnd : sqlFormula -> sqlFormula -> sqlFormula
+  | sqlOr : sqlFormula -> sqlFormula -> sqlFormula
+  | sqlNot : sqlFormula -> sqlFormula
+  | sqlExists : sql -> sqlFormula
+  with
+  sql :=
+  | sqlQuery : list sqlExpr -> list (sqlTableExpr * var) -> sqlFormula -> sql
+  with
+  sqlTableExpr :=
+  | sqlTable : table -> sqlTableExpr
+  | sqlSelect : sql -> sqlTableExpr
+  .
+
+  Program Instance sqlFormulaS : Setoid sqlFormula.
+  
+  Inductive sqlStmt :=
+  | sqlQueryStmt : sql -> sqlStmt
+  | sqlInsertStmt : table -> sql -> sqlStmt
+  | sqlUpdateStmt : table -> colind -> sqlExpr -> sqlFormula -> sqlStmt
+  | sqlDeleteStmt : table -> sqlFormula -> sqlStmt
+  .
+
+  Program Instance sqlStmtS : Setoid sqlStmt.
+  
+End SQLSyntax.
+
+Section SQLExprInductionPrinciple.
+  Variables (p : sqlExpr -> Prop) (Q : list sqlExpr -> Prop).
+
+  Hypothesis
+    (pval : forall val, p (sqlValExpr val))
+    (pvar : forall var, p (sqlVarExpr var))
+    (pcol : forall e, p e -> forall col, p (sqlColExpr e col))
+    (papp0 : Q List.nil)
+    (papp1 : forall e, p e -> forall l, Q l -> Q (e :: l))
+    (papp : forall builtin l, Q l -> p (sqlAppExpr builtin l)).
+  
+    Fixpoint sqlExpr_ind_2 e : p e :=
+    match e as x return p x with
+      | sqlValExpr val => pval val
+      | sqlVarExpr var => pvar var
+      | sqlColExpr e col => pcol e (sqlExpr_ind_2 e) col
+      | sqlAppExpr builtin l =>
+        papp builtin l ((
+               fix dep_fold_right (l' : list sqlExpr) : Q l' :=
+                 match l' as x return Q x with
+                   | List.nil => papp0
+                   | e :: es => papp1 e (sqlExpr_ind_2 e) es (dep_fold_right es)
+                 end
+             ) l)
+    end.
+End SQLExprInductionPrinciple.
+
+Section SQLSemanticsDefs.
+  Definition row := lista nat.
+  Instance rowS : Setoid row := listaS natS.
+  Definition col := lista (maybe nat).
+  Instance colS : Setoid col := listaS (maybeS natS).
+  Definition rowind := nat.
+  Definition database := list (matrixp nat). 
+  Instance databaseS : Setoid database := listS (matrixpS natS).
+  Definition store := FMapNat.t sqlVal.
+
+
+  Section Getters.
+
+    Definition _cellGetter t ri ci := previewS @ (nthTraversal @ t ∘ matrixCellTraversal ri ci).
+
+    Instance _cellGetter_Proper : Proper (equiv ==> equiv ==> equiv ==> equiv) _cellGetter.
+    Proof.
+      solve_proper.
+    Qed.
+
+    Definition cellGetter := injF3 _cellGetter _.
+
+    Existing Instance ConstMaybeFunctor.
+    Existing Instance ConstMaybe_Applicative.
+
+    Definition _rowGetter t (ri: rowind) : databaseS ~> maybeS (rowS) := previewS @ (nthTraversal @ t ∘ matrixRowTraversal ri).
+
+    Instance _rowGetter_Proper : Proper (equiv ==> equiv ==> equiv) _rowGetter.
+    Proof.
+      solve_proper.
+    Qed.
+
+    Definition rowGetter := injF2 _rowGetter _.
+
+    Definition _colGetter t (ci: colind) : databaseS ~>  maybeS (colS) :=
+      previewS @ (nthTraversal @ t ∘ matrixColLens @ ci). 
+
+    Instance _colGetter_Proper : Proper (equiv ==> equiv ==> equiv) _colGetter.
+    Proof.
+      solve_proper.
+    Qed.
+
+    Definition colGetter := injF2 _colGetter _.
+
+    Definition _rowsGetter t : databaseS ~> maybeS (listaS (maybeS (rowS))) := previewS @ (nthTraversal @ t ∘ matrixRowsLens).
+
+    Instance _rowsGetter_Proper : Proper (equiv ==> equiv) _rowsGetter.
+    Proof.
+      solve_proper.
+    Qed.
+
+    Definition rowsGetter := injF _rowsGetter _.
+
+    Definition _tableGetter t : databaseS ~> maybeS (matrixpS natS) := previewS @ (nthTraversal @ t).
+
+    Instance _tableGetter_Proper : Proper (equiv ==> equiv) _tableGetter.
+    Proof.
+      solve_proper.
+    Qed.
+
+    Definition tableGetter := injF _tableGetter _.
+
+    Definition _widthGetter t : databaseS ~> maybeS (natS) :=
+      previewS @ (nthTraversal @ t ∘ matrixWidthLens).
+
+    Instance _widthGetter_Proper : Proper (equiv ==> equiv) _widthGetter.
+    Proof.
+      solve_proper.
+    Qed.
+
+    Definition widthGetter := injF _widthGetter _.
+
+    Definition tableRowsGetter : matrixpS natS ~> listaS (maybeS (rowS)) := view (matrixRowsLens).
+
+    Definition tableWidthGetter : matrixpS natS ~>  (natS) :=
+      view (matrixWidthLens).
+
+    Definition tableCellGetter ri ci : matrixpS natS ~> (maybeS natS) :=
+      previewS @ (matrixCellTraversal ri ci).
+    
+    Lemma ConstIso_iso : forall A B (AS : Setoid A) (BS : Setoid B) (a : B),
+            match ConstIsoS BS AS @ a with
+              | ConstIso _ _ a' => a'
+            end = a.
+    Proof.
+      auto.
+    Qed.
+
+    Lemma ConstIso'_iso : forall A B (AS : Setoid A) (BS : Setoid B) a,
+            ConstIso B A (ConstIso' B A a) = a.
+    Proof.
+      intros. destruct a. auto. 
+    Qed.
+
+    Definition _maybeRowGetter (t: table) (ri: rowind) : databaseS ~>  maybeS (maybeS rowS) :=
+      previewS @ (nthTraversal @ t ∘ matrixRowsLens ∘ listaNthLens ri). 
+
+    Instance _maybeRowGetter_Proper : Proper (equiv ==> equiv ==> equiv) _maybeRowGetter.
+    Proof.
+      autounfold. intros. unfold _maybeRowGetter. rewritesr.
+    Qed.
+
+    Definition maybeRowGetter := injF2 _maybeRowGetter _.
+
+    Section CellGetter_comp.
+      Opaque matrixCellTraversal.
+    Lemma cellGetter_comp :
+      forall t ri ci h,
+        (tableGetter @ t @ h) >>= tableCellGetter ri ci = cellGetter @ t @ ri @ ci @ h.
+    Proof.
+      intros. generalize t h. clear t h. double induction t h.
+      - reflexivity.
+      - intros. Opaque equiv pre0. simpl. unfold _maybe_first_mappend. Transparent pre0. unfold pre0 at 1 2. Opaque pre0. simpl.
+        match goal with
+          | |- ?a = match ?b with _ => _ end => let H:=fresh "H" in assert (a = b) as H; [auto | rewrite H; destruct b; [reflexivity | reflexivity ] ] 
+        end
+          .
+      - intros. simpl. reflexivity.
+      - intros. Opaque equiv pre0. simpl in *. unfold _nthTraversal, _nthTraversal' in *. simpl in *. rewrite ConstIso'_iso. rewrite ConstIso'_iso. apply H0. 
+    Qed.
+
+    End CellGetter_comp.
+
+  End Getters.
+  
+  Section Setters.
+    Existing Instance ConstMaybeFunctor.
+    Existing Instance ConstMaybe_Applicative.
+
+    Existing Instance IdentityFunctor.
+    Existing Instance Identity_Applicative.
+
+    Definition _cellSetter t (ri: rowind) (ci: colind) (n : nat) : databaseS ~> databaseS :=
+      setS @ (nthTraversal @ t ∘ matrixCellTraversal ri ci) @ n.
+
+    Instance _cellSetter_Proper : Proper (equiv ==> equiv ==> equiv ==> equiv ==> equiv) _cellSetter.
+    Proof.
+      solve_proper.
+    Qed.
+
+    Definition cellSetter := injF4 _cellSetter _.
+    
+    Definition _rowSetter t (ri: rowind) (r : row) : databaseS ~> databaseS :=
+      setS @ (nthTraversal @ t ∘ matrixRowTraversal ri) @ r.
+
+    Instance _rowSetter_Proper : Proper (equiv ==> equiv ==> equiv ==> equiv) _rowSetter.
+    Proof.
+      autounfold. intros. unfold _rowSetter, set. rewritesr. 
+    Qed.
+
+    Definition rowSetter := injF3 _rowSetter _.
+    
+    Definition _maybeRowSetter (t: table) (ri: rowind) (r : maybe row) : databaseS ~>  databaseS :=
+      setS @ (nthTraversal @ t ∘ matrixRowsLens ∘ listaNthLens ri) @ r. 
+
+    Instance _maybeRowSetter_Proper : Proper (equiv ==> equiv ==> equiv ==> equiv) _maybeRowSetter.
+    Proof.
+      autounfold. intros. unfold _maybeRowSetter, set. rewritesr.
+    Qed.
+
+    Definition maybeRowSetter := injF3 _maybeRowSetter _.
+
+    Definition _rowsSetter (t: table) (rows : lista (maybe row)) : databaseS ~>  databaseS :=
+      setS @ (nthTraversal @ t ∘ matrixRowsLens) @ rows.
+
+    Instance _rowsSetter_Proper : Proper (equiv ==> equiv ==> equiv) _rowsSetter.
+    Proof.
+      autounfold. intros. unfold _rowsSetter, set. rewritesr.
+    Qed.
+
+    Definition rowsSetter := injF2 _rowsSetter _.
+     
+  End Setters.
+  
+  Instance FMapNat_Equal_Equivalence A : Equivalence (@FMapNat.Equal A).
+  Proof.
+    split.
+    autounfold. unfold FMapNat.Equal. intros. reflexivity.
+    autounfold. unfold FMapNat.Equal. intros. symmetry. auto.
+    autounfold. unfold FMapNat.Equal. intros. transitivity (FMapNat.find y0 y). auto. auto.
+  Qed.
+  
+  Instance FMapNatSetoid A : Setoid (FMapNat.t A) :=
+    {
+      equiv := @FMapNat.Equal A
+    }.
+  
+
+  Instance storeS : Setoid store := FMapNatSetoid sqlVal.  
+  Definition colLookup val colind : option nat :=
+    match val with
+      | vRow row =>     nth_error row colind
+      | _ => None
+    end
+  .
+
+  Definition storeProd (s1 s2 : store) : store :=
+    FMapNat.fold (fun k e s => FMapNat.add k e s) s1 s2.
+  
+  Definition storesProd (ss1 ss2 : list store) : list store :=
+    concat (map (fun s => map (fun s2 => storeProd s s2) ss2) ss1).
+
+End SQLSemanticsDefs.
+
