SQL/SQLHeap.v
@@ -1,0 +1,608 @@
+Require Import Definitions Algebra.Monoid Expr Algebra.SetoidCat Algebra.Maybe Tactics Algebra.ListUtils Algebra.Functor Algebra.Applicative Algebra.Alternative Algebra.FoldableFunctor Algebra.PairUtils Algebra.Maybe Algebra.Monad Algebra.Lens.Lens Algebra.Lens.MaybeLens ListLens Utils SetoidUtils SQL Pointed SQLUtils.
+Require Import Coq.Structures.DecidableTypeEx List SetoidClass PeanoNat FMapWeakList Basics Coq.Arith.Compare_dec Coq.Arith.Le.
+
+
+Definition insertRow table (h : database) : database :=
+  match rowsGetter @ table @ h with
+    | None => h
+    | Some rows => maybeRowSetter @ table @ (lista_findaS maybe_row_eq_dec @ rows) @ (SomeS @ (lista_repeatS @ 0)) @ h
+  end.
+
+Instance insertRow_Proper : Proper (equiv ==> equiv ==> equiv) insertRow.
+Proof.
+  autounfold. intros. unfold insertRow. matchequiv. simpl in H1. rewrite H, H0, H1. reflexivity. auto. 
+Qed.
+
+Definition insertRowS : tableS ~> databaseS ~~> databaseS := injF2 insertRow _.
+
+Definition deleteRow table rowid (h : database) : database :=
+  match rowsGetter @ table @ h with
+    | None => h
+    | Some rows => maybeRowSetter @ table @ rowid @ None @ h
+  end.
+
+Instance deleteRow_Proper : Proper (equiv ==> equiv ==> equiv ==> equiv) deleteRow.
+Proof.
+  autounfold. intros. unfold deleteRow. matchequiv. rewritesr. auto. 
+Qed.
+
+Definition deleteRowS : tableS ~> natS ~~> databaseS ~~> databaseS := injF3 deleteRow _.
+
+Definition newRowId table (h : database) : option nat :=
+  match rowsGetter @ table @ h with
+    | None => None
+    | Some rows => SomeS @ (lista_findaS maybe_row_eq_dec @ rows)
+  end.
+
+Instance newRowId_Proper : Proper (equiv ==> equiv ==> equiv) newRowId.
+Proof.
+  autounfold. intros. unfold newRowId. matchequiv. simpl in H1. rewrite H1. reflexivity.
+Qed.
+
+Definition newRowIdS : tableS ~> databaseS ~~> maybeS natS := injF2 newRowId _.
+
+Open Scope nat_scope.
+
+Definition addrToTable addr (h : database) : table :=
+  addr mod (length h).
+
+Definition addrToRow addr (h : database) : nat :=
+  addr / length h.
+
+Instance addrToTable_Proper : Proper (equiv ==> equiv ==> equiv) addrToTable.
+Proof.
+  autounfold. intros. unfold addrToTable. rewritesr.  
+Qed.
+
+Definition addrToTableS : natS ~> databaseS ~~> tableS := injF2 addrToTable _.
+
+Instance addrToRow_Proper : Proper (equiv ==> equiv ==> equiv) addrToRow.
+Proof.
+  autounfold. intros. unfold addrToRow. rewritesr.  
+Qed.
+
+Definition addrToRowS : natS ~> databaseS ~~> natS := injF2 addrToRow _.
+
+Fixpoint _predToTable n t (pred1 : pred) (db : database) : maybe (table * colind) :=
+  match db with
+    | nil => None
+    | tab :: tabs =>
+      let (n2, rs) := tab in
+      if lt_dec pred1 (n + n2) then
+        Some (t, pred1 - n)
+      else
+        _predToTable (n + n2) (t + 1) pred1 tabs
+  end
+.
+
+Instance _predToTable_Proper : Proper (equiv ==> equiv ==> equiv ==> equiv ==> equiv) _predToTable.
+Proof.
+  autounfold. intros. rewrite H1. clear H1 x1. generalize x y H x0 y0 H0 y1 H2. clear x y H x0 y0 H0 y1 H2. apply list_ind_2 with (l1:=x2) (l2:=y2).
+  intros. simpl. auto.
+  intros. inversion H2.
+  intros. inversion H2.
+  intros. inversion H2. unfold _predToTable. fold _predToTable. destruct a, c.  destruct H6. rewrite H6, H0. destruct (lt_dec y1  (y + n0)). rewritesr. apply H. rewritesr. rewritesr. auto.
+Qed.
+
+Definition predToTableS : predS ~> databaseS ~~> maybeS tableS.
+  simple refine (injF2 (fun pred1 db => fstS <$> _predToTable 0 0 pred1 db) _).
+  exact (@maybeS).
+  apply monadFunctor.
+  Lemma predToTable_1 : Proper (equiv ==> equiv ==> equiv)
+                               (fun (pred1 : pred) (db : database) =>
+                                  fstS <$> _predToTable 0 0 pred1 db).
+  Proof.
+    solve_proper.
+  Qed.
+  apply predToTable_1.
+Defined.
+
+Definition predToColS : predS ~> databaseS ~~> maybeS natS.
+  simple refine (injF2 (fun pred1 db => sndS <$> _predToTable 0 0 pred1 db) _).
+  exact (@maybeS).
+  apply monadFunctor.
+  Lemma predToCol_1 : Proper (equiv ==> equiv ==> equiv)
+                             (fun (pred1 : pred) (db : database) =>
+                                sndS <$> _predToTable 0 0 pred1 db).
+  Proof.
+    solve_proper.
+  Qed.
+  apply predToCol_1.
+Defined.      
+
+Import SQLValType.
+
+
+Definition getNewAddr (type1 : type) (h : database) : maybe nat.
+  simple refine (newRowIdS @ type1 @ h >>= injF (fun rowid => ret @ (rowid * (length h) + type1)) _).
+Defined.
+
+Definition noneFalse : boolS ~> maybeS unitS :=
+  injF (fun b : bool => if b then ret @ tt else None) _.
+
+Definition fromMaybeS {A} {AS : Setoid A} : AS ~> maybeS AS ~~> AS.
+  simple refine (injF2 (fun a b => match b with
+                                     | Some b' => b'
+                                     | None => a
+                                   end) _).
+  Lemma fromMaybeS_1 : forall {A} {AS : Setoid A}, Proper (equiv ==> equiv ==> equiv)
+     (fun (a : A) (b : option A) =>
+      match b with
+      | Some b' => b'
+      | None => a
+      end).
+  Proof.
+    autounfold. intros. matchequiv. auto. auto.
+  Qed.
+  apply fromMaybeS_1.
+Defined.
+
+
+Definition eqbS := injF2 Nat.eqb _.
+
+Definition checkAddrPred addr pred1 h :=
+  (eqbS
+     @ (addrToTableS @ addr @ h)
+     <$> (predToTableS @ pred1 @ h) ) >>=
+                                      noneFalse.
+
+Definition _newAddr (type1 : type) h :=
+  pairS
+    @ (insertRowS @ type1 @ h)
+    <$> (vNatS <$> getNewAddr type1 h).
+
+Definition newAddr : typeS ~> databaseS ~~> maybeS (databaseS ~*~ valS).
+  simple refine (injF2 _newAddr _).
+  Lemma newAddr_1 : Proper (equiv ==> equiv ==> equiv) _newAddr.
+  Proof.
+    autounfold. intros. unfold _newAddr, getNewAddr. evalproper. rewritesr. evalproper. bindproper. rewritesr. rewritesr.
+  Qed.
+  apply newAddr_1.
+Defined.
+
+Definition _filterByCol ci val1 row  :=
+  match nth_error row ci, extractNatS @ val1 with
+    | Some n, Some n' => eqbS @ n @ n'
+    | _, _ => false
+  end.
+
+Instance _filterByCol_Proper : Proper (equiv ==> equiv ==> equiv ==> equiv) _filterByCol.
+Proof.
+  autounfold. intros. unfold _filterByCol. matchequiv. matchequiv. rewritesr.
+Qed.
+
+Definition filterByCol := injF3 _filterByCol _.
+
+Definition _filterVal val1 val2  :=
+  match val2, extractNatS @ val1 with
+    | Some n, Some n' => eqbS @ n @ n'
+    | _, _ => false
+  end.
+
+Instance _filterVal_Proper : Proper (equiv ==> equiv ==> equiv) _filterVal.
+Proof.
+  autounfold. intros. unfold _filterVal. matchequiv. matchequiv. rewritesr.
+Qed.
+
+Definition filterVal := injF2 _filterVal _.
+
+(*
+  Definition _filterNone {A} {AS : Setoid A} (val1 : maybe A)  :=
+    match val1 with
+      | Some n => true
+      | None => false
+    end.
+
+  Instance _filterNone_Proper A AS : Proper (equiv ==> equiv) (@_filterNone A AS).
+  Proof.
+    autounfold. intros. unfold _filterNone. matchequiv. 
+  Qed.
+
+  Definition filterNone {A AS} := injF (@_filterNone A AS) _.
+ *)
+
+Definition _getAddr (h : database) t ri  : nat  :=
+  ri * length h + t.
+
+Instance _getAddr_Proper : Proper (equiv ==> equiv ==> equiv ==> equiv) _getAddr.
+Proof.
+  autounfold. intros. unfold _getAddr. rewritesr. 
+Qed.
+
+Definition getAddr := injF3 _getAddr _.
+
+Definition _lookupByObject pred1 val1 h : list sqlVal :=
+  match predToTableS @ pred1 @ h, predToColS @ pred1 @ h with
+    | Some t, Some ci =>
+      match colGetter @ t @ ci @ h with
+        | Some col =>
+          mapS
+            @ (vNatS ∘ getAddr @ h @ t)
+            @ (lista_filter_indexS @ (filterVal @ val1) @ col )
+        | None => nil                  
+      end
+    | _, _ => nil
+  end.
+
+Lemma _predToTable_le : forall n t pred1 m, _predToTable n t pred1 m = None \/ (exists a b, _predToTable n t pred1 m = Some (a, b) /\ a >= t).
+    intros. generalize  n t pred1. clear n t pred1.   induction m. left. auto.
+    intros. destruct a.  simpl. destruct (lt_dec pred1 (n + n0)). right. exists t. exists (pred1 - n). auto.  pose (IHm (n+n0) (t+1) pred1). destruct o. tauto. right. destruct H as [? [? ?]]. exists x. exists x0. split. tauto. destruct H. unfold ge in *. apply le_Sn_le. rewrite plus_symmetry in H0.  auto.
+Qed.
+
+Module SQLHeap <: Heap SQLValType.
+  
+  Definition t := database.
+  Program Instance tS : Setoid t.
+
+  Definition _delete0 addr h : t := deleteRowS
+                                    @ (addrToTableS @ addr @ h)
+                                    @ (addrToRowS @ addr @ h)
+                                    @ h.
+
+  
+  Instance _delete0_Proper : Proper (equiv ==> equiv ==> equiv) _delete0.
+  Proof.
+    autounfold. intros. unfold _delete0. rewritesr. 
+  Qed.
+
+  Definition delete0 : natS ~> tS ~~>  tS := injF2 _delete0 _.
+
+  Definition _delete addr h :=
+    fromMaybeS @ h @ (delete0 <$> extractNatS @ addr <*> pure @ h).
+
+  Instance _delete_Proper : Proper (equiv ==> equiv ==> equiv) _delete.
+  Proof.
+    autounfold. intros. unfold _delete. rewritesr.
+  Qed.
+
+  Definition delete := injF2 _delete _.
+
+  Definition _read0 addr pred1 h : maybe nat :=
+    checkAddrPred addr pred1 h >>
+                  (cellGetter
+                     @ (addrToTableS @ addr @ h)
+                     @ (addrToRowS @ addr @ h)
+                     <$> predToColS @ pred1 @ h
+                     <*> pure @ h : maybe (maybe nat)) >>= fmap @ idS.
+
+  Instance _read0_Proper : Proper (equiv ==> equiv ==> equiv ==> equiv) _read0.                     
+  Proof.
+    autounfold. intros. unfold _read0, checkAddrPred. rewritesr. 
+  Qed.
+
+  Definition read0 := injF3 _read0 _.
+
+  Definition _read addr pred1 h : maybe sqlVal :=
+    (read0 <$> extractNatS @ addr <*> pure @ pred1 <*> pure @ h : maybe (maybe nat)) >>= fmap @ vNatS.
+  
+  Instance _read_Proper : Proper (equiv ==> equiv ==> equiv ==> equiv) _read.                     
+  Proof.
+    autounfold. intros. unfold _read. rewritesr. 
+  Qed.
+
+  Definition read : valS ~> predS ~~> tS ~~> maybeS valS := injF3 _read _.
+  
+  Definition _update0 addr pred1 val1 h : maybe t :=
+    checkAddrPred addr pred1 h >>
+                  (cellSetter
+                     @ (addrToTableS @ addr @ h)
+                     @ (addrToRowS @ addr @ h)
+                     <$> predToColS @ pred1 @ h
+                     <*> pure @ val1 
+                     <*> pure @ h).
+  
+  Instance _update0_Proper : Proper (equiv ==> equiv ==> equiv ==> equiv ==> equiv) _update0.
+  Proof.
+    autounfold. intros. unfold _update0, checkAddrPred. rewritesr. 
+  Qed.
+
+  Definition update0 := injF4 _update0 _.
+
+  Definition _update addr pred1 val1 h : t :=
+    fromMaybeS @ h @ ((update0 <$> extractNatS @ addr <*> pure @ pred1 <*> extractNatS @ val1 <*> pure @ h) >>= fmap @ idS).
+
+  Instance _update_Proper : Proper (equiv ==> equiv ==> equiv ==> equiv ==> equiv) _update.
+  Proof.
+    autounfold. intros. unfold _update. rewritesr. 
+  Qed.
+
+  Definition update : valS ~> predS ~~> valS ~~> tS ~~> tS := injF4 _update _.
+  
+  Definition emptyH : database := nil.
+  Definition union : tS ~> tS ~~> tS := unionDatabases.
+
+  Definition _allocated0 addr h : Prop :=
+    match fromMaybeS @ None @ (maybeRowGetter
+                                 @ (addrToTableS @ addr @ h)
+                                 @ (addrToRowS @ addr @ h)
+                                 @ h) with
+      | None => False
+      | Some _ => True
+    end.
+
+  Instance _allocated0_Proper : Proper (equiv ==> equiv==>equiv) _allocated0.
+  Proof.
+    autounfold. intros. unfold _allocated0. matchequiv.
+  Qed.
+
+  Definition allocated0 := injF2 _allocated0 _.
+  
+  Definition _allocated addr h :=
+    match allocated0
+            <$> extractNatS @ addr
+            <*> pure @ h with
+      | None => False
+      | Some a => a
+    end
+  .
+  
+  Instance _allocated_Proper : Proper (equiv ==> equiv==>equiv) _allocated.
+  Proof.
+    autounfold. intros. unfold _allocated. matchequiv. auto.
+  Qed.
+
+  Definition allocated := injF2 _allocated _.
+
+  Definition l A (AS : Setoid A) := list A.
+  Instance lS A (AS : Setoid A) : Setoid (l A AS) := listS AS.
+  Instance func : @Functor l lS := listFunctor.
+  Instance alt : @Alternative l lS := list_Alternative.
+  Instance foldable : @FoldableFunctor l lS func := list_Foldable.
+  Instance app : @Applicative l lS func := list_Applicative.
+
+  Definition _lookupBySPO addr pred1 val1 h :=
+    match read @ addr @ pred1 @ h with
+      | None => false
+      | Some val2 =>         
+        if SQLValType.equiv_dec val1 val2 then true else false
+    end
+  .
+
+  Instance _lookupBySPO_Proper : Proper (equiv ==> equiv ==> equiv ==> equiv ==> equiv) _lookupBySPO.
+  Proof.
+    autounfold. intros. unfold _lookupBySPO. matchequiv. rewritesr. 
+  Qed.
+
+  Definition lookupBySPO :  valS ~> predS ~~> valS ~~> tS ~~> boolS := injF4 _lookupBySPO _.
+
+  Instance _lookupByObject_Proper : Proper (equiv ==> equiv ==> equiv ==> equiv) _lookupByObject.
+  Proof.
+    autounfold. intros. unfold _lookupByObject. matchequiv. matchequiv. matchequiv. simpl in H2, H3, H4. rewrite H0, H1, H2, H4. reflexivity.
+  Qed.
+
+  Definition lookupByObject   : predS ~> valS ~~> tS ~~> lS _ valS := injF3 _lookupByObject _.
+  
+  Definition _lookupByPred pred1 h : list (sqlVal * sqlVal) :=
+    match predToTableS @ pred1 @ h, predToColS @ pred1 @ h with
+      | Some t, Some ci =>
+        match colGetter @ t @ ci @ h with
+          | Some col =>
+            mapS
+              @ ((vNatS ∘ getAddr @ h @ t) *** vNatS)
+              @ (lista_filter_indexS' @ col)
+          | None => nil                  
+        end
+      | _, _ => nil
+    end.
+
+  Instance _lookupByPred_Proper : Proper (equiv ==> equiv ==> equiv) _lookupByPred.
+  Proof.
+    autounfold. intros. unfold _lookupByPred. matchequiv. matchequiv. matchequiv. simpl in H1, H2, H3. rewrite H0, H1, H3. reflexivity.
+  Qed.
+
+  Definition lookupByPred   : predS ~> tS ~~> lS _ (valS ~*~ valS) := injF2 _lookupByPred _. 
+
+  Definition _predOfType pred1 type1 h :=
+    match predToTableS @ pred1 @ h with
+      | None => False
+      | Some t' => type1 == t'
+    end.
+
+  Instance _predOfType_Proper : Proper (equiv ==> equiv ==> equiv ==> equiv) _predOfType.
+  Proof.
+    autounfold. intros. unfold _predOfType. matchequiv. simpl in H2. rewrite H0, H2. reflexivity.
+  Qed.
+
+  Definition predOfType :
+    predS ~> typeS ~~> databaseS ~~> iff_setoid := injF3 _predOfType _.
+  
+  Definition _typeOfHeap type1 (h : database) :=
+    type1 < length h.
+
+  Instance _typeOfHeap_Proper : Proper (equiv ==> equiv ==> equiv) _typeOfHeap.
+  Proof.
+    autounfold. intros. unfold _typeOfHeap. rewrite H, H0. reflexivity.
+  Qed.
+
+  Definition typeOfHeap : typeS  ~> databaseS ~~> iff_setoid := injF2 _typeOfHeap _.    
+             
+  Notation "heap [ val , pred ]" := (read @ val @ pred @ heap) (at level 11).
+  Notation "heap [ val , pred  ↦  val2 ]  " := (update @ val @ pred @ val2 @ heap) (at level 11).
+
+  Require Import Coq.Arith.Minus.
+  
+
+  Lemma _read_cons_1 :
+    forall addr pred1 table1 h ,
+      pred1 < _width table1 ->
+      addrToTable addr (table1 :: h) = 0 ->
+      _read0 addr pred1 (table1 :: h) == tableCellGetter (addrToRow addr (table1 :: h)) pred1 @ table1.
+  Proof.
+    intros. unfold _read0.
+    assert (checkAddrPred addr pred1 (table1 :: h) == Some tt).
+    {
+      unfold checkAddrPred, addrToTableS. normalize. rewrite H0. unfold predToTableS. normalize. unfold _predToTable. destruct table1. simpl (0+n). destruct (lt_dec pred1 n). simpl. auto.
+      tauto. 
+    }
+    rewrite H1. unfold addrToTableS. normalize. rewrite H0. unfold predToColS.    normalize. destruct table1. unfold _predToTable. simpl (0 + _).  destruct (lt_dec pred1 n).
+    - assert (forall A (AS : Setoid A) (x : A), Some x == ret @ x).
+    {
+      reflexivity.
+    }
+    rewrite H2. unfold andThen, compM.  normalizecomp. unfold constS. normalize. rewrite associativity. rewrite left_unit. normalize. simpl  (sndS <$> Some (0, pred1 - 0)). rewrite <- (minus_n_O pred1). unfold addrToRowS. normalize. generalize (addrToRow addr (matrixpCons nat n l0 :: h)). intros.
+    simpl fmap. unfold monad_fmap. normalizecomp. unfold ap. unfold comp2S. normalize. rewrite uncurry_fmap_prod. rewrite fmap_eval.
+    assert (forall A (AS : Setoid A) (x : A), Some x == ret @ x).
+    {
+      reflexivity.
+    }
+    rewrite H3. rewrite left_unit. normalize. 
+    assert (forall A (AS : Setoid A) (x : A), (ret @ x : maybe A) == pure @ x).
+    {
+      reflexivity.
+    }
+    rewrite H4. rewrite ap_pure. rewrite fmap_pure. rewrite <- cellGetter_comp. rewrite <- H4.  normalize_monad.
+    simpl (tableGetter @ 0 @ (matrixpCons nat n l0 :: h)). rewrite H3.
+    match goal with
+      | |- ret @ ?a >>= ?f == _ =>
+        rewrite (left_unit _ _ _ _ a f)
+    end. normalize.
+    match goal with
+      | |- ?a >>= ?f == _ =>
+        rewrite (right_unit_equiv _ _ _ a f)
+    end.
+    reflexivity. simpl. arrequiv.
+    
+  - tauto.
+    Grab Existential Variables.
+    solve_proper.
+  Qed.
+  
+    
+  Lemma eq_heap :
+    forall (h1 h2 : t) ,
+      (forall v, allocated @ v @ h1 == allocated @ v @ h2) ->
+      (forall v p, read @ v @ p @ h1 == read @ v @ p @ h2) ->
+      (forall p t, predOfType @ p @ t @ h1 <-> predOfType @ p @ t @ h2) ->
+      (forall t, typeOfHeap @ t @ h1 <-> typeOfHeap @ t @ h2) ->
+      h1 == h2.
+  Proof.
+    
+    intros. generalize H H0 H1 H2. clear H H0 H1 H2. apply list_ind_2 with (l1:=h1)(l2:=h2).
+    -    reflexivity.
+    - intros. pose (H3 0).    simpl in i . unfold _typeOfHeap in i. simpl in i.  assert (0 < S (length b)).  apply le_n_S. apply Nat.le_0_l.  destruct i. pose (H6 H4). inversion l0. 
+    - intros. pose (H3 0).    simpl in i . unfold _typeOfHeap in i. simpl in i.  assert (0 < S (length b)).  apply le_n_S. apply Nat.le_0_l.  destruct i. pose (H5 H4). inversion l0. 
+    - intros. constructor. destruct a, c.
+      + destruct (lt_eq_lt_dec n n0) as [[? | ?] | ?].
+        * destruct n0. inversion l2.
+          specialize (H2 n0 0). simpl in H2. unfold _predOfType in H2. simpl in H2. assert False. clear H3 H0 H. destruct (lt_dec n0 n) , (lt_dec n0 (S n0)).
+          apply (nat_int _ _ l2 l3).
+          apply (nat_int _ _ l2 l3).
+          destruct b. simpl in H1. tauto. pose (_predToTable_le n 1 n0 (m::b)). destruct o. rewrite H in H2. apply H2. auto. destruct H as [? [? [? ?]]]. rewrite H in H2. simpl in H2. destruct H2. rewrite <- H3 in H0. inversion H0. auto.
+          apply n2. constructor.
+          tauto. 
+        * rewrite e in *. clear n e. clear H H2 H3. split. auto. destruct l0, l1. unfold _rows. generalize H0 H1. clear H0 H1. apply list_ind_2 with (l1:=l0) (l2:=l1).
+          {
+            intros. induction n0.
+            {
+              destruct o, o0.
+              {
+                simpl. destruct l2, l3.  simpl. auto.
+              }
+              {
+                Opaque equiv _read0.  simpl in e. unfold _read in e. simpl in e. destruct l2, l3. Transparent equiv. induction n0.
+              {
+                simpl.  auto.
+              }
+              {
+                simpl. auto.
+                simpl in e. unfold lista_equiv0. 
+
+pose (_read_cons_1 0 0 (matrixpCons nat n0 (listaCons (option (lista nat)) (Some l2) nil)) b).
+
+              assert (_read0 0 0
+       (matrixpCons nat n0 (listaCons (option (lista nat)) (Some l2) nil)
+        :: b) == rewrite uncurry_fmap_prod. rewrite uncurry_fmap_prod. rewrite uncurry_fmap_prod. rewrite fmap_eval. rewrite fmap_eval. rewrite fmap_eval. unfold ap. normalize_monad. unfold comp2S. normalizecomp. normalize_monad.
+              unfold injF3 in e. unfold injF2 in e. simpl in e. unfold monad_fmap in e. normalize_monad. simpl in e.
+              pose _read_cons_1. assert (exists a', _read0 0 0
+          (matrixpCons nat n0 (listaCons (option (lista nat)) (Some l2) nil)
+                       :: b) = Some a').
+              {
+                
+                rewrite _read_cons_1 in e. rewritesr. simpl. simpl in H0. destruct H0.
+           pose (nat_int _ _ l2).
+          simpl in H1. destruct m, (lt_dec n0 (n + n2)). destruct H1. simpl in H0. assert (0 = 0). auto. pose (H0 H1). inversion e. destruct H0. auto. tauto.
+          unfold _predToTable in H1. destruct b.
+          apply (nat_int _ _ l2 l3).
+          pose (H2 0).    simpl in i . unfold _typeOfHeap in i. simpl in i.  assert (0 < S (length b)).  apply le_n_S. apply Nat.le_0_l.  destruct i. pose (H5 H3). inversion l0. 
+
+  Axiom dom_lookup : forall h val,  inDom @ val @ h -> exists pred val2, h [val,pred] == Some val2.
+
+  Axiom dom_domPred : forall h val, inDom @ val @ h -> exists pred, inPredDom @ val @ pred @ h.
+
+  Axiom domPred_lookup : forall h val pred, inPredDom @ val @ pred @ h -> exists val2, h[val, pred] == Some val2.
+
+  Axiom lookupBySubject_empty : forall val pred, emptyH [val,pred] == None.
+
+  Axiom lookupByObject_empty : forall pred val, lookupByObject @ pred @ val @ emptyH == empty.
+
+  Axiom lookupByPred_empty : forall pred , lookupByPred @ pred @ emptyH == empty.
+
+  Axiom lookupBySPO_empty : forall val pred val2, lookupBySPO @ val @ pred @ val2 @ emptyH == false.
+  
+  Axiom lookup_predDom : forall h val pred, (exists val2, lookupBySubject @ val @ pred @ h == Some val2) ->  inPredDom @ val @ pred @ h.
+
+  Axiom predDom_dom : forall h val, (exists pred, inPredDom @ val @ pred @ h) -> inDom @ val @ h.
+
+  Lemma lookup_dom : forall h val, (exists pred val2, lookupBySubject @ val @ pred @ h == Some val2) -> inDom @ val @ h.
+  Proof.
+    intros. apply predDom_dom. destruct H as [? [? ?]]. exists x. apply lookup_predDom. exists x0.  auto.
+  Qed.
+
+  Axiom predDom_newAddr:
+        forall h h' val pred, (h', val) == newAddr @ h -> ~ inPredDom @ val @ pred @ h.
+  
+  Axiom lookupBySubject_predDom_0:
+        forall h val pred, ~ inPredDom @ val @ pred @ h -> h [val , pred] == None.
+  
+  Axiom lookupBySubject_predDom_1:
+        forall h val pred, inPredDom @ val @ pred @ h -> exists val2, h [val , pred] == val2.
+
+  Lemma lookupBySubject_newAddr:
+        forall h h' val pred, (h', val) == newAddr @ h -> h [val, pred] == None.
+  Proof.
+    intros. apply lookupBySubject_predDom_0. apply predDom_newAddr with (h:=h) (h':=h'). auto.
+  Qed.
+  
+  Axiom lookup_update :
+    forall h val pred val2,
+      h [ val , pred ↦  val2 ] [ val , pred ] == Some val2.
+  
+  Axiom lookup_update_diff_addr :
+    forall h val val' pred pred' val2,
+      val <> val' ->
+      h [ val , pred ↦ val2 ] [ val' , pred' ] == h [ val' , pred' ].
+  
+  Axiom lookup_update_diff_pred :
+    forall h val val' pred pred' val2,
+      pred <> pred' ->
+      h [ val , pred ↦ val2 ] [ val' , pred' ] == h [ val' , pred' ].
+  
+  Axiom update_update :
+    forall h val pred val2 val3,
+      h [ val , pred ↦  val2 ] [ val , pred ↦ val3 ] == h  [ val , pred ↦ val3 ].
+  
+  Axiom predDom_update :
+    forall h val pred val2,
+       inPredDom @ val @ pred @ ( h [ val , pred ↦ val2 ]).
+  
+  Axiom predDom_update_diff_addr :
+    forall h val val' pred pred' val2,
+      val <> val' -> 
+      inPredDom @ val @ pred @ ( h [ val' , pred' ↦ val2 ]) == inPredDom @ val @ pred @ h.
+
+  Axiom predDom_update_diff_pred :
+    forall h val val' pred pred' val2,
+      pred <> pred' -> 
+      inPredDom @ val @ pred @ ( h [ val' , pred' ↦ val2 ]) == inPredDom @ val @ pred @ h.
+
+  Axiom dom_update_diff_addr :
+    forall h val val' pred val2,
+      val <> val' -> 
+      inDom @ val @ ( h [ val' , pred ↦ val2 ]) == inDom @ val @ h.
+
+
+
+
+
+
+End SQLHeap.
