SQL/SQLSemantics.v
@@ -1,0 +1,124 @@
+Require Import Assert Command Definitions Algebra.Monoid Expr Algebra.SetoidCat Algebra.Maybe Tactics Algebra.ListUtils Algebra.Functor Algebra.Applicative Algebra.Alternative Algebra.FoldableFunctor Algebra.PairUtils Algebra.Maybe Algebra.Monad Algebra.Lens Utils SetoidUtils SQLStore SQLHeap.
+Require Import Coq.Structures.DecidableTypeEx List SetoidClass PeanoNat FMapWeakList Basics.
+
+Module SQLBuiltInExpr <: BuiltInExpr SQLValType.
+  Definition builtInExpr := sqlBuiltIn.
+  Definition builtInExprS := natS.
+  Definition appBIE : builtInExprS ~> listS SQLValType.valS ~~> optionS SQLValType.valS :=
+    constS _ @ (constS _ @ None).
+End SQLBuiltInExpr.
+
+Module SQLBuiltInFormula <: BuiltInFormula SQLValType SQLStore SQLHeap.
+  Definition builtInFormula := sqlFormula.
+  Instance builtInFormulaS : Setoid builtInFormula := sqlFormulaS.
+  Definition appBIE : sqlFormulaS ~> listS sqlValS ~~> databaseS ~~> storeS ~~> listS storeS :=
+  constS _ @ (constS _ @ (constS _ @ constS _ @ nil)).
+End SQLBuiltInFormula.
+      
+Module SQLModel .
+  (* SQL as builtInFormula and builtInCommand *)
+  Fixpoint sqlExprEval (s : store) (e : sqlExpr) : option sqlVal :=
+    match e with
+      | sqlValExpr val => Some val
+      | sqlVarExpr var => FMapNat.find var s
+      | sqlColExpr e colind =>
+        match sqlExprEval s e with
+          | Some val =>
+            match colLookup val colind with
+              | Some n => Some (vNat n)
+              | None => None
+            end
+          | None => None
+        end
+      | sqlAppExpr builtin args =>
+        match sequence (map (sqlExprEval s) args) with
+          | Some l => SQLBuiltInExpr.appBIE @ builtin @ l
+          | None => None
+        end
+    end
+  .
+
+
+    Fixpoint sqlFormEval (s : store) (m : database) (form: sqlFormula) : option bool :=
+      match form with
+        | sqlBuiltIn builtin args =>
+          match sequence (map (sqlExprEval s) args) with
+            | Some l => BP.app @ builtin @ l
+            | None => None
+          end
+        | sqlAnd form1 form2 =>
+          match sqlFormEval s m form1 with
+            | Some b1 =>
+              match sqlFormEval s m form2 with
+                | Some b2 => Some (andb b1 b2)
+                | None => None
+              end
+            | None => None
+          end
+        | sqlOr form1 form2 =>
+          match sqlFormEval s m form1 with
+            | Some b1 =>
+              match sqlFormEval s m form2 with
+                | Some b2 => Some (orb b1 b2)
+                | None => None
+              end
+            | None => None
+          end
+        | sqlNot form1 =>
+          match sqlFormEval s m form1 with
+            | Some b1 => Some (negb b1)
+            | None => None
+          end
+        | sqlExists sql =>
+          match sqlReduce s m sql with
+            | Some l => Some (null l)
+            | None => None
+          end
+      end
+    with
+    sqlReduce (s : store) (m : database) (sql1 : sql) : option resultSet :=
+      match sql1 with
+        | sqlQuery rets tabs form =>
+          match sequence (map (fun tab : sqlTableExpr * var =>
+                                 let (te, var) := tab in
+                                 match (sqlTableExprEval s m te) with
+                                   | Some rs => Some (map (fun r => singleton var (vRow r)) rs)
+                                   | None => None
+                                 end) tabs) with
+            | Some l =>
+              let ss := fold_left storesProd l (s :: List.nil) in
+              match sequence (map (fun s =>
+                                     match sqlFormEval s m form with
+                                       | Some b => if b then Some (s::List.nil) else Some List.nil 
+                                       | _ => None
+                                     end) ss) with
+                | Some ss' =>
+                  let filtered := concat ss' in
+                  sequence (map (fun s =>
+                                   sequence (map (fun (e : sqlExpr) =>
+                                                    match sqlExprEval s e with
+                                                      | Some val =>
+                                                        match val with
+                                                          | vNat nat => Some nat
+                                                          | _ => None
+                                                        end     
+                                                      | None => None
+                                                    end
+                                             ) rets) ) filtered)
+                | None => None
+              end
+            | None => None
+          end
+      end
+    with
+    sqlTableExprEval (s : store) (m : database) (te : sqlTableExpr) : option resultSet :=
+      match te with
+        | sqlTable tab => match (nth_error m tab) with
+                            | Some tab => Some (snd tab)
+                            | None => None
+                          end
+        | sqlSelect sql1 => sqlReduce s m sql1
+      end
+    .
+    
+End SQLModel.
