SQL/SQLUtils.v
@@ -1,0 +1,221 @@
+Require Import Definitions Algebra.Monoid Expr Algebra.SetoidCat Algebra.Maybe Tactics Algebra.ListUtils Algebra.Functor Algebra.Applicative Algebra.Alternative Algebra.FoldableFunctor Algebra.PairUtils Algebra.Maybe Algebra.Monad Algebra.Lens.Lens Algebra.Lens.MaybeLens ListLens Utils SetoidUtils SQL Pointed.
+Require Import Coq.Structures.DecidableTypeEx List SetoidClass PeanoNat FMapWeakList Basics Coq.Arith.Compare_dec.
+
+Existing Instance maybe_Monad.
+Instance maybeFunctor : @Functor maybe (@maybeS) := monadFunctor.
+Instance maybe_Applicative : @Applicative maybe (@maybeS) _ := monad_Applicative.
+  
+(*  (* based on https://github.com/bacam/coqjvm/blob/master/coqjvm/ListExt.v *)
+  Fixpoint list_update {A:Type} {AS : Setoid A} (l:list A) (n:nat) (t:A -> maybe A) {struct n} : maybe (list A) :=
+  match n, l with
+    | 0,   old_v::rest => match t old_v with
+                            | None => None
+                            | Some v => Some (v::rest)
+                          end
+  | S n, v'::rest    => match list_update rest n t with None => None | Some rest' => Some (v'::rest') end
+  | _,   nil         => None
+  end.
+
+  Instance listUpdate_Proper A (AS : Setoid A): Proper (equiv ==> equiv ==> (equiv ==> equiv) ==> equiv) (@list_update A AS).
+  Proof.
+    autounfold. intros. rewrite H0.  clear x0 H0. generalize y0 H. clear H. apply list_ind_2 with (l1:=x) (l2:=y).
+    intros. induction y2.
+    simpl. auto.
+    simpl. auto.
+    intros. inversion H0.
+    intros. inversion H0.
+    intros. inversion H0. induction y2.
+    simpl. assert (x1 a == y1 c). apply H1. auto. destruct (x1 a), (y1 c). constructor. auto. auto. inversion H8. inversion H8. auto.
+    simpl. assert (list_update b y2 x1 == list_update d y2 y1). apply H. auto. destruct (list_update b y2 x1), (list_update d y2 y1). constructor. auto. auto. inversion H8. inversion H8. auto.
+  Qed.
+
+  Fixpoint list_update' {A:Type} (l:list A) (n:nat) (t:A ->  A) {struct n} :  list A :=
+  match n, l with
+    | 0,   old_v::rest => t old_v::rest
+  | S n, v'::rest    =>  v'::list_update' rest n t 
+  | _,   nil         => nil
+  end.
+
+  Instance listUpdate'_Proper A (AS : Setoid A): Proper (equiv ==> equiv ==> (equiv ==> equiv) ==> equiv) (@list_update' A).
+  Proof.
+    autounfold. intros. rewrite H0.  clear x0 H0. generalize y0 H. clear H. apply list_ind_2 with (l1:=x) (l2:=y).
+    intros. induction y2.
+    simpl. auto.
+    simpl. auto.
+    intros. inversion H0.
+    intros. inversion H0.
+    intros. inversion H0. induction y2.
+    simpl. assert (x1 a == y1 c). apply H1. auto. constructor. auto. auto. 
+    simpl. constructor. auto. apply H. auto.
+  Qed.
+ *)
+
+
+Existing Instance list_A_Monoid.
+
+Definition _maybe_mappend {C} {CS : Setoid C} {mon : @Monoid C CS} (a b : maybe C) : maybe C :=
+  match a with
+    | None => b
+    | Some a' => match b with
+                   | None => a
+                   | Some b' => Some (mappend @ a' @ b')
+                 end
+  end
+.
+
+Instance _maybe_mappend_Proper {C} {CS : Setoid C} {mon : @Monoid C CS} : Proper (equiv ==> equiv ==> equiv) _maybe_mappend.
+Proof.
+  autounfold. intros. unfold _maybe_mappend. matchequiv. matchequiv. simpl in *. rewritesr.  auto. auto.
+Qed.
+
+Definition maybe_mappend {C} {CS : Setoid C} {mon : @Monoid C CS}: maybeS CS ~> maybeS CS ~~> maybeS CS := injF2 _maybe_mappend _.
+      
+Instance maybe_A_Monoid {C} {CS : Setoid C} {mon : @Monoid C CS}: @Monoid (maybe C) _.
+Proof.
+  exists (None) (maybe_mappend).
+  intros. simpl. destruct a. reflexivity. auto.
+  intros. simpl. destruct a. simpl. reflexivity. simpl. auto.
+  intros. simpl. destruct a. simpl. destruct b. simpl. destruct c. rewrite associativity_monoid. reflexivity. reflexivity. destruct c. simpl. reflexivity. simpl. reflexivity. destruct b. simpl. destruct c. reflexivity. reflexivity. destruct c. simpl. reflexivity. simpl. auto.
+Defined.
+
+
+Definition unionRows : listaS (maybeS rowS) ~> listaS (maybeS rowS) ~~> listaS (maybeS rowS) :=
+  lista_zipWithS @ mappend.
+
+Definition minS := injF2 min _.
+
+Definition _unionTables (tab1 tab2 : matrixp nat) : matrixp nat :=
+  matrixpConsS @ (minS @ (tableWidthGetter @ tab1) @ (tableWidthGetter @ tab2)) @ (unionRows @ (tableRowsGetter @ tab1) @ (tableRowsGetter @ tab2)).
+
+Instance _unionTables_Proper : Proper (equiv ==> equiv ==> equiv) _unionTables.
+Proof.
+  autounfold. intros. unfold _unionTables. rewritesr.
+Qed.
+
+Definition unionTables := injF2 _unionTables _.
+
+Definition unionDatabases : databaseS ~> databaseS ~~> databaseS :=
+  list_zipWithS' @ unionTables.
+
+Fixpoint list_maybe_filter {A : Type} {AS : Setoid A} (p : AS ~> boolS) (l : list (maybe A)) : list A :=
+    match l with
+      | nil => nil
+      | None :: l' => list_maybe_filter p l'
+      | Some a :: l' => if p @ a then a :: list_maybe_filter p l' else list_maybe_filter p l'
+    end.
+
+Instance list_maybe_filter_Proper A (AS : Setoid A) : Proper (equiv ==> equiv ==> equiv) (@list_maybe_filter A AS).
+  Proof.
+    autounfold. intros. generalize H0. clear H0. apply list_ind_2 with (l1:=x0) (l2:=y0).
+    intros. reflexivity.
+    intros. inversion H1.
+    intros. inversion H1.
+    intros. inversion H1. simpl. matchequiv. simpl in H8. rewrites. destruct (y @ a0). constructor. auto. apply H0.  auto. apply H0. auto. apply H0. auto.
+  Qed.
+  
+Fixpoint list_maybe_filter_index {A : Type} {AS : Setoid A} n (p : AS ~> boolS) (l : list (maybe A)) : list nat :=
+    match l with
+      | nil => nil
+      | None :: l' => list_maybe_filter_index (S n) p l'
+      | Some a :: l' => if p @ a then n :: list_maybe_filter_index (S n) p l' else list_maybe_filter_index (S n) p l'
+    end.
+
+Instance list_maybe_filter_index_Proper A (AS : Setoid A) : Proper (equiv ==> equiv ==> equiv ==> equiv) (@list_maybe_filter_index A AS).
+Proof.
+    autounfold. intros. generalize H1 x y H . clear H x y H1. apply list_ind_2 with (l1:=x1) (l2:=y1).
+    intros. reflexivity.
+    intros. inversion H1.
+    intros. inversion H1.
+    intros. inversion H1. simpl. matchequiv. simpl in H9. rewrite H0, H9. destruct (y0 @ a0). constructor. auto. apply H.  auto. rewritesr. apply H. auto. rewritesr. apply H. auto. rewritesr.
+Qed.
+
+Fixpoint list_maybe_filter_index' {A : Type} {AS : Setoid A} n (p : AS ~> boolS) (l : list (maybe A)) : list (nat * A) :=
+    match l with
+      | nil => nil
+      | None :: l' => list_maybe_filter_index' (S n) p l'
+      | Some a :: l' => if p @ a then (n,a) :: list_maybe_filter_index' (S n) p l' else list_maybe_filter_index' (S n) p l'
+    end.
+
+Instance list_maybe_filter_index'_Proper A (AS : Setoid A) : Proper (equiv ==> equiv ==> equiv ==> equiv) (@list_maybe_filter_index' A AS).
+Proof.
+    autounfold. intros. generalize H1 x y H . clear H x y H1. apply list_ind_2 with (l1:=x1) (l2:=y1).
+    intros. reflexivity.
+    intros. inversion H1.
+    intros. inversion H1.
+    intros. inversion H1. simpl. matchequiv. simpl in H9. rewrite H0, H9. destruct (y0 @ a0). constructor. auto. apply H.  auto. rewritesr. apply H. auto. rewritesr. apply H. auto. rewritesr.
+Qed.
+
+Fixpoint duplicate {A} (n : nat) (a : A) : list A :=
+  match n with
+    | 0 => nil
+    | S n => a :: duplicate n a
+  end.
+
+Definition extractNat  (val1 : sqlVal)  : maybe nat :=
+  match val1 with
+    | vNat n => Some n
+    | _ => None
+  end.
+  
+Instance extractNat_Proper : Proper (equiv ==> equiv) extractNat.
+Proof.
+  autounfold. intros. unfold extractNat.  matchequiv.  inversion H. rewritesr. inversion H. inversion H. 
+Qed.
+  
+Definition extractNatS : sqlValS ~> maybeS natS := injF extractNat _.
+
+
+Instance vNat_Proper : Proper (equiv ==> equiv) vNat.
+Proof.
+  solve_proper.    
+Qed.
+
+Definition vNatS : natS ~> sqlValS := injF vNat _.
+
+Instance pair_Proper A B (AS : Setoid A) (BS : Setoid B): Proper (equiv ==> equiv ==> equiv) (@pair A B).
+Proof.
+  autounfold. intros. split. auto. auto.
+Qed.
+
+
+Lemma maybe_row_eq_dec : forall r1 r2 : maybe row, {r1 == r2} + {~r1 == r2}.
+  intros.  destruct r1, r2.
+  - destruct r, r0. destruct (Nat.eq_dec n n0).
+    + apply list_rect_2 with (l1:=l) (l2:=l0).
+      * left. rewrite e. reflexivity.
+      * intros. destruct H.
+        destruct e0. destruct (Nat.eq_dec a n).
+        rewrite <- e, e0. left. simpl. auto.
+        right. simpl. tauto.
+        right. simpl in *. tauto.
+      * intros. destruct H.
+        destruct (Nat.eq_dec a n0).
+        rewrite e, e1. left. rewrite e in e0. simpl. auto.
+        right. simpl. tauto.
+        right. simpl in *. tauto.
+      * intros. destruct H.
+        destruct (Nat.eq_dec a c).
+        rewrite <- e, e1. left. simpl in *. rewrite <- e in e0. auto.
+        right. simpl. tauto.
+        right. simpl in *. tauto.
+    + right. intro. apply n1. assert (n == n0). apply listaCons_equiv with (l1:=l)(l2:=l0). auto. auto.
+  - right. intro. inversion H.
+  - right. intro. inversion H.
+  - left. reflexivity.
+Qed.
+
+  Lemma nat_int : forall n n' , n < S n' -> ~ n' < n.
+  Proof.
+    double induction n n'.
+    intros. intro. inversion H0.
+    intros. intro. inversion H0. inversion H1.
+    intros. intro. inversion H0. inversion H3.
+    intros. intro. apply H0 with (n':=n0). apply le_S_n. auto. apply le_S_n. auto.
+  Qed.
+
+  Open Scope nat_scope.
+  Lemma plus_symmetry : forall a b, a+b = b+a.
+  Proof.
+    induction a. intros. simpl. apply plus_n_O.
+    intros. simpl. rewrite <- plus_n_Sm. f_equal. apply IHa.
+  Qed.
